SyBloc/SBSemantics.v
@@ -29,570 +29,357 @@ environment.
    *)
 
   Definition state := memory val.
-  Definition evolution := memory (stream val).
+  (* Definition evolution := memory (stream val). *)
 
   Definition transient_states := PM.t state.
-  Definition transient_evolutions := PM.t evolution.
+  (* Definition transient_evolutions := PM.t evolution. *)
 
 
   Definition env := PM.t value.
-  Definition history := PM.t (stream value).
+  (* Definition history := PM.t (stream value). *)
 
   (** ** Instantaneous semantics *)
 
-  Section InstantSemantics.
+  Section ExprSemantics.
 
     Variable base: bool.
     Variable R: env.
     Variable S: state.
     (* Variable Ts: transient_states. *)
 
-    Inductive sem_var_var_instant: ident -> value -> Prop :=
+    Inductive sem_var_var: ident -> value -> Prop :=
       Svv:
         forall x v,
           PM.find x R = Some v ->
-          sem_var_var_instant x v.
+          sem_var_var x v.
 
-    Inductive sem_clock_instant: clock -> bool -> Prop :=
+    Inductive sem_clock: clock -> bool -> Prop :=
     | Sbase:
-        sem_clock_instant Cbase base
+        sem_clock Cbase base
     | Son:
         forall ck x c b,
-          sem_clock_instant ck true ->
-          sem_var_instant ck x (present c) ->
+          sem_clock ck true ->
+          sem_var ck x (present c) ->
           val_to_bool c = Some b ->
-          sem_clock_instant (Con ck x b) true
+          sem_clock (Con ck x b) true
     | Son_abs1:
         forall ck x c,
-          sem_clock_instant ck false ->
-          sem_var_instant ck x absent ->
-          sem_clock_instant (Con ck x c) false
+          sem_clock ck false ->
+          sem_var ck x absent ->
+          sem_clock (Con ck x c) false
     | Son_abs2:
         forall ck x c b,
-          sem_clock_instant ck true ->
-          sem_var_instant ck x (present c) ->
+          sem_clock ck true ->
+          sem_var ck x (present c) ->
           val_to_bool c = Some b ->
-          sem_clock_instant (Con ck x (negb b)) false
+          sem_clock (Con ck x (negb b)) false
 
-    with sem_state_var_instant: clock -> ident -> value -> Prop :=
+    with sem_state_var: clock -> ident -> value -> Prop :=
          | SsvPresent:
              forall x v ck,
                find_val x S = Some v ->
-               sem_clock_instant ck true ->
-               sem_state_var_instant ck x (present v)
+               sem_clock ck true ->
+               sem_state_var ck x (present v)
          | SsvAbsent:
              forall x ck,
                find_val x S <> None ->
-               sem_clock_instant ck false ->
-               sem_state_var_instant ck x absent
+               sem_clock ck false ->
+               sem_state_var ck x absent
 
-    with sem_var_instant: clock -> var -> value -> Prop :=
+    with sem_var: clock -> var -> value -> Prop :=
          | Sv:
              forall x v ck,
-               sem_var_var_instant x v ->
-               sem_var_instant ck (Var x) v
+               sem_var_var x v ->
+               sem_var ck (Var x) v
          | Sl:
              forall x v ck,
-               sem_state_var_instant ck x v ->
-               sem_var_instant ck (Last x) v.
+               sem_state_var ck x v ->
+               sem_var ck (Last x) v.
 
-    Scheme sem_clock_instant_mut := Induction for sem_clock_instant Sort Prop
-             with sem_state_var_instant_mut := Induction for sem_state_var_instant Sort Prop
-             with sem_var_instant_mut := Induction for sem_var_instant Sort Prop.
+    Scheme sem_clock_mut := Induction for sem_clock Sort Prop
+             with sem_state_var_mut := Induction for sem_state_var Sort Prop
+             with sem_var_mut := Induction for sem_var Sort Prop.
 
     Combined Scheme sem_clock_state_var_var_mut from
-             sem_clock_instant_mut, sem_state_var_instant_mut, sem_var_instant_mut.
+             sem_clock_mut, sem_state_var_mut, sem_var_mut.
 
-    Definition sem_vars_instant (xs: idents) (vs: list value) : Prop :=
-      Forall2 sem_var_var_instant xs vs.
+    Definition sem_vars (xs: idents) (vs: list value) : Prop :=
+      Forall2 sem_var_var xs vs.
 
-    Inductive sem_lexp_instant: clock -> lexp -> value -> Prop:=
+    Inductive sem_lexp: clock -> lexp -> value -> Prop:=
     | Sconst:
         forall c v ck,
           v = (if base then present (sem_const c) else absent) ->
-          sem_lexp_instant ck (Econst c) v
+          sem_lexp ck (Econst c) v
     | Svar:
         forall x v ty ck,
-          sem_var_instant ck x v ->
-          sem_lexp_instant ck (Evar x ty) v
+          sem_var ck x v ->
+          sem_lexp ck (Evar x ty) v
     | Swhen_eq:
         forall s x sc xc b ck,
-          sem_var_instant ck x (present xc) ->
-          sem_lexp_instant ck s (present sc) ->
+          sem_var ck x (present xc) ->
+          sem_lexp ck s (present sc) ->
           val_to_bool xc = Some b ->
-          sem_lexp_instant (Con ck x b) (Ewhen s x b) (present sc)
+          sem_lexp (Con ck x b) (Ewhen s x b) (present sc)
     | Swhen_abs1:
         forall s x sc xc b ck,
-          sem_var_instant ck x (present xc) ->
+          sem_var ck x (present xc) ->
           val_to_bool xc = Some b ->
-          sem_lexp_instant ck s (present sc) ->
-          sem_lexp_instant (Con ck x (negb b)) (Ewhen s x (negb b)) absent
+          sem_lexp ck s (present sc) ->
+          sem_lexp (Con ck x (negb b)) (Ewhen s x (negb b)) absent
     | Swhen_abs:
         forall s x b ck,
-          sem_var_instant ck x absent ->
-          sem_lexp_instant ck s absent ->
-          sem_lexp_instant (Con ck x b) (Ewhen s x b) absent
+          sem_var ck x absent ->
+          sem_lexp ck s absent ->
+          sem_lexp (Con ck x b) (Ewhen s x b) absent
     | Sunop_eq:
         forall le op c c' ty ck,
-          sem_lexp_instant ck le (present c) ->
+          sem_lexp ck le (present c) ->
           sem_unop op c (typeof le) = Some c' ->
-          sem_lexp_instant ck (Eunop op le ty) (present c')
+          sem_lexp ck (Eunop op le ty) (present c')
     | Sunop_abs:
         forall le op ty ck,
-          sem_lexp_instant ck le absent ->
-          sem_lexp_instant ck (Eunop op le ty) absent
+          sem_lexp ck le absent ->
+          sem_lexp ck (Eunop op le ty) absent
     | Sbinop_eq:
         forall le1 le2 op c1 c2 c' ty ck,
-          sem_lexp_instant ck le1 (present c1) ->
-          sem_lexp_instant ck le2 (present c2) ->
+          sem_lexp ck le1 (present c1) ->
+          sem_lexp ck le2 (present c2) ->
           sem_binop op c1 (typeof le1) c2 (typeof le2) = Some c' ->
-          sem_lexp_instant ck (Ebinop op le1 le2 ty) (present c')
+          sem_lexp ck (Ebinop op le1 le2 ty) (present c')
     | Sbinop_abs:
         forall le1 le2 op ty ck,
-          sem_lexp_instant ck le1 absent ->
-          sem_lexp_instant ck le2 absent ->
-          sem_lexp_instant ck (Ebinop op le1 le2 ty) absent.
+          sem_lexp ck le1 absent ->
+          sem_lexp ck le2 absent ->
+          sem_lexp ck (Ebinop op le1 le2 ty) absent.
 
-    Definition sem_lexps_instant (ck: clock) (les: list lexp) (vs: list value) :=
-      Forall2 (sem_lexp_instant ck) les vs.
+    Definition sem_lexps (ck: clock) (les: list lexp) (vs: list value) :=
+      Forall2 (sem_lexp ck) les vs.
 
-    Inductive sem_cexp_instant: clock -> cexp -> value -> Prop :=
+    Inductive sem_cexp: clock -> cexp -> value -> Prop :=
     | Smerge_true:
         forall x t f c ck,
-          sem_var_instant ck x (present true_val) ->
-          sem_cexp_instant (Con ck x true) t (present c) ->
-          sem_cexp_instant (Con ck x false) f absent ->
-          sem_cexp_instant ck (Emerge x t f) (present c)
+          sem_var ck x (present true_val) ->
+          sem_cexp (Con ck x true) t (present c) ->
+          sem_cexp (Con ck x false) f absent ->
+          sem_cexp ck (Emerge x t f) (present c)
     | Smerge_false:
         forall x t f c ck,
-          sem_var_instant ck x (present false_val) ->
-          sem_cexp_instant (Con ck x true) t absent ->
-          sem_cexp_instant (Con ck x false) f (present c) ->
-          sem_cexp_instant ck (Emerge x t f) (present c)
+          sem_var ck x (present false_val) ->
+          sem_cexp (Con ck x true) t absent ->
+          sem_cexp (Con ck x false) f (present c) ->
+          sem_cexp ck (Emerge x t f) (present c)
     | Smerge_abs:
         forall x t f ck,
-          sem_var_instant ck x absent ->
-          sem_cexp_instant (Con ck x true) t absent ->
-          sem_cexp_instant (Con ck x false) f absent ->
-          sem_cexp_instant ck (Emerge x t f) absent
+          sem_var ck x absent ->
+          sem_cexp (Con ck x true) t absent ->
+          sem_cexp (Con ck x false) f absent ->
+          sem_cexp ck (Emerge x t f) absent
     | Site_eq:
         forall x t f c b ct cf ck,
-          sem_lexp_instant ck x (present c) ->
-          sem_cexp_instant ck t (present ct) ->
-          sem_cexp_instant ck f (present cf) ->
+          sem_lexp ck x (present c) ->
+          sem_cexp ck t (present ct) ->
+          sem_cexp ck f (present cf) ->
           val_to_bool c = Some b ->
-          sem_cexp_instant ck (Eite x t f) (if b then present ct else present cf)
+          sem_cexp ck (Eite x t f) (if b then present ct else present cf)
     | Site_abs:
         forall b t f ck,
-          sem_lexp_instant ck b absent ->
-          sem_cexp_instant ck t absent ->
-          sem_cexp_instant ck f absent ->
-          sem_cexp_instant ck (Eite b t f) absent
+          sem_lexp ck b absent ->
+          sem_cexp ck t absent ->
+          sem_cexp ck f absent ->
+          sem_cexp ck (Eite b t f) absent
     | Sexp:
         forall e v ck,
-          sem_lexp_instant ck e v ->
-          sem_cexp_instant ck (Eexp e) v.
+          sem_lexp ck e v ->
+          sem_cexp ck (Eexp e) v.
 
-  End InstantSemantics.
-
-  Section InstantAnnotatedSemantics.
-
-    Variable base : bool.
-    Variable R: env.
-    Variable S: state.
-
-    Inductive sem_annotated_instant {A}
-              (sem_instant: bool -> env -> state -> clock -> A -> value -> Prop)
+    Inductive sem_annotated {A}
+              (sem: clock -> A -> value -> Prop)
       : clock -> A -> value -> Prop :=
     | Stick:
         forall ck a c,
-          sem_instant base R S ck a (present c) ->
-          sem_clock_instant base R S ck true ->
-          sem_annotated_instant sem_instant ck a (present c)
+          sem ck a (present c) ->
+          sem_clock ck true ->
+          sem_annotated sem ck a (present c)
     | Sabs:
         forall ck a,
-          sem_instant base R S ck a absent ->
-          sem_clock_instant base R S ck false ->
-          sem_annotated_instant sem_instant ck a absent.
+          sem ck a absent ->
+          sem_clock ck false ->
+          sem_annotated sem ck a absent.
 
-    Definition sem_laexp_instant := sem_annotated_instant sem_lexp_instant.
-    Definition sem_caexp_instant := sem_annotated_instant sem_cexp_instant.
+    Definition sem_laexp := sem_annotated sem_lexp.
+    Definition sem_caexp := sem_annotated sem_cexp.
 
-    Inductive sem_laexps_instant: clock -> list lexp -> list value -> Prop:=
+    Inductive sem_laexps: clock -> list lexp -> list value -> Prop:=
     | SLticks:
         forall ck ces cs vs,
           vs = map present cs ->
-          sem_lexps_instant base R S ck ces vs ->
-          sem_clock_instant base R S ck true ->
-          sem_laexps_instant ck ces vs
+          sem_lexps ck ces vs ->
+          sem_clock ck true ->
+          sem_laexps ck ces vs
     | SLabss:
         forall ck ces vs,
           vs = all_absent ces ->
-          sem_lexps_instant base R S ck ces vs ->
-          sem_clock_instant base R S ck false ->
-          sem_laexps_instant ck ces vs.
+          sem_lexps ck ces vs ->
+          sem_clock ck false ->
+          sem_laexps ck ces vs.
 
-  End InstantAnnotatedSemantics.
+  End ExprSemantics.
 
-  (** ** Liftings of instantaneous semantics *)
-
-  Section LiftSemantics.
-
-    Variable bk : stream bool.
-    Variable H : history.
-    Variable E : evolution.
-
-    Definition sample {A} (n: nat) (xs: stream A) := xs n.
-    Hint Unfold sample.
-
-    Definition restr_evol (n: nat): state :=
-      mmap (sample n) E.
-
-    Definition restr_hist (n: nat): env :=
-      PM.map (sample n) H.
-    Hint Unfold restr_hist.
-
-    Definition lift {A B} (sem: bool -> env -> state -> clock -> A -> B -> Prop)
-               ck x (ys: stream B): Prop :=
-      forall n, sem (bk n) (restr_hist n) (restr_evol n) ck x (ys n).
-    Hint Unfold lift.
-
-    Definition lift' {A B} (sem: env -> state -> clock -> A -> B -> Prop) ck x (ys: stream B): Prop :=
-      forall n, sem (restr_hist n) (restr_evol n) ck x (ys n).
-    Hint Unfold lift'.
-
-    Definition lift'' {A B} (sem: env -> clock -> A -> B -> Prop) ck x (ys: stream B): Prop :=
-      forall n, sem (restr_hist n) ck x (ys n).
-    Hint Unfold lift''.
-
-    Definition lift''' {A B} (sem: state -> clock -> A -> B -> Prop) ck x (ys: stream B): Prop :=
-      forall n, sem (restr_evol n) ck x (ys n).
-    Hint Unfold lift'''.
-
-    Definition lift'''' {A B} (sem: bool -> env -> state -> A -> B -> Prop)
-               x (ys: stream B): Prop :=
-      forall n, sem (bk n) (restr_hist n) (restr_evol n) x (ys n).
-    Hint Unfold lift''''.
-
-    Definition lift''''' {A B} (sem: env -> A -> B -> Prop)
-               x (ys: stream B): Prop :=
-      forall n, sem (restr_hist n) x (ys n).
-    Hint Unfold lift'''''.
-    (* Definition lift''' {A B} (sem: bool -> env -> A -> B -> Prop) x (ys: stream B): Prop := *)
-    (*   forall n, sem (bk n) (restr_hist n) x (ys n). *)
-    (* Hint Unfold lift'''. *)
-
-    Definition sem_clock (ck: clock) (xs: stream bool): Prop :=
-      lift'''' sem_clock_instant ck xs.
-
-    Definition sem_var ck (x: var) (xs: stream value): Prop :=
-      lift sem_var_instant ck x xs.
-
-    (* Definition sem_last (x: ident) (xs: stream value): Prop := *)
-    (*   lift'' sem_last_instant x xs. *)
-
-    Definition sem_var_var (x: ident) (xs: stream value): Prop :=
-      lift''''' sem_var_var_instant x xs.
-
-    Definition sem_state_var ck (x: ident) (xs: stream value): Prop :=
-      lift sem_state_var_instant ck x xs.
-
-    Definition sem_vars (x: idents) (xs: stream (list value)): Prop :=
-      lift''''' sem_vars_instant x xs.
-
-    Definition sem_laexp ck (e: lexp) (xs: stream value): Prop :=
-      lift'''' (fun base R S => sem_laexp_instant base R S ck) e xs.
-
-    Definition sem_laexps (ck: clock) (e: list lexp) (xs: stream (list value)): Prop :=
-      lift'''' (fun base R S => sem_laexps_instant base R S ck) e xs.
-
-    Definition sem_lexp ck (e: lexp) (xs: stream value): Prop :=
-      lift sem_lexp_instant ck e xs.
-
-    Definition sem_lexps ck (e: list lexp) (xs: stream (list value)): Prop :=
-      lift sem_lexps_instant ck e xs.
-
-    Definition sem_caexp ck (c: cexp) (xs: stream value): Prop :=
-      lift'''' (fun base R S => sem_caexp_instant base R S ck) c xs.
-
-    Definition sem_cexp ck (c: cexp) (xs: stream value): Prop :=
-      lift sem_cexp_instant ck c xs.
-
-  End LiftSemantics.
-
-  (** ** Time-dependent semantics *)
-
-  Definition instant_same_clock (l : list value) : Prop :=
-    absent_list l \/ present_list l.
-
-  Definition same_clock (l_s : stream (list value)) : Prop :=
-    forall n, instant_same_clock (l_s n).
-
-  Definition clock_of (xss: stream (list value))(bs: stream bool): Prop :=
-    forall n,
-      present_list (xss n) <-> bs n = true.
-
-  Definition clock_of' (xss: stream (list value)) : stream bool :=
-    fun n => forallb (fun v => negb (v ==b absent)) (xss n).
-
-  Lemma clock_of_equiv:
-    forall xss, clock_of xss (clock_of' xss).
-  Proof.
-    split; intros H.
-    - unfold clock_of'.
-      rewrite forallb_forall.
-      intros; rewrite Bool.negb_true_iff.
-      rewrite not_equiv_decb_equiv.
-      eapply In_Forall in H; eauto.
-    - unfold clock_of' in H.
-      rewrite forallb_forall in H.
-      apply all_In_Forall; intros ** Hin E.
-      specialize (H _ Hin).
-      rewrite Bool.negb_true_iff, not_equiv_decb_equiv in H.
-      apply H; eauto.
-  Qed.
-
-  Lemma clock_of_equiv':
-    forall xss bk,
-      clock_of xss bk ->
-      bk ≈ clock_of' xss.
-  Proof.
-    intros ** H n; specialize (H n).
-    unfold clock_of'.
-    induction (xss n) as [|v]; simpl.
-    - apply H; constructor.
-    - destruct v.
-      + simpl.
-        rewrite <-Bool.not_true_iff_false, <-H.
-        inversion 1; auto.
-      + simpl.
-        apply IHl; rewrite <-H.
-        split; intro P.
-        * constructor; auto.
-          intro; discriminate.
-        * inv P; auto.
-  Qed.
-
-  (* Record mvalues := *)
-  (*   Mvalues { content: stream val; *)
-  (*             reset: stream bool *)
-  (*           }. *)
-
-  (* (* Definition memory := RMemory.memory mvalue. *) *)
-  (* Definition memories := RMemory.memory mvalues. *)
-
-  (* Inductive reset_regs: stream bool -> memories -> Prop := *)
-  (*   reset_regs_intro: *)
-  (*     forall M rs, *)
-  (*       (forall x mvs, *)
-  (*           find_val x M = Some mvs -> *)
-  (*           forall n, rs n = true -> mvs.(reset) n = true) -> *)
-  (*       (forall x M', *)
-  (*           sub_inst x M M' -> *)
-  (*           reset_regs rs M') -> *)
-  (*       reset_regs rs M. *)
-
-  (* (* Definition next (n: nat) (mvs: mvalues) (v0 v: val) : Prop := *) *)
-  (* (*   mvs.(content) (S n) = (if mvs.(reset) (S n) then v0 else v). *) *)
-
-  (* (* Inductive fby_spec: nat -> val -> value -> mvalues -> value -> Prop := *) *)
-  (* (* | fby_spec_present: *) *)
-  (* (*     forall n v0 v mvs, *) *)
-  (* (*       next n mvs v0 v -> *) *)
-  (* (*       fby_spec n v0 (present v) mv (mv.(content) n) *) *)
-  (* (* | fby_spec_absent: *) *)
-  (* (*     forall n v0 v mvs, *) *)
-  (* (*       next n mvs v0 (mvs.(content) n) -> *) *)
-  (* (*       fby_spec n v0 absent mvs absent. *) *)
-
-  (* Inductive mfby: ident -> val -> stream value -> memories -> stream value -> Prop := *)
-  (*   mfby_intro: *)
-  (*     forall x mvs v0 ls M xs, *)
-  (*       find_val x M = Some mvs -> *)
-  (*       mvs.(content) 0 = v0 -> *)
-  (*       (forall n, match ls n with *)
-  (*             | absent => *)
-  (*               mvs.(content) (S n) = (if mvs.(reset) (S n) then v0 else mvs.(content) n) *)
-  (*               /\ xs n = absent *)
-  (*             | present v => *)
-  (*               mvs.(content) (S n) = (if mvs.(reset) (S n) then v0 else v) *)
-  (*               /\ xs n = present (mvs.(content) n) *)
-  (*             end) -> *)
-  (*       mfby x v0 ls M xs. *)
-
-  (* Definition fby_eq (mems: PS.t) (eq: equation) : PS.t := *)
-  (*   match eq with *)
-  (*   | EqFby x _ _ _ => PS.add x mems *)
-  (*   | _ => mems *)
-  (*   end. *)
-
-  (* Definition fbys (eqs: list equation) : PS.t := *)
-  (*   fold_left fby_eq eqs PS.empty. *)
-
-  (* Definition inst_eq (insts: PS.t) (eq: equation) : PS.t := *)
-  (*   match eq with *)
-  (*   | EqReset _ _ i _ => PS.add i insts *)
-  (*   | EqCall _ _ _ i _ => PS.add i insts *)
-  (*   | _ => insts *)
-  (*   end. *)
-
-  (* Definition insts (eqs: list equation) : PS.t := *)
-  (*   fold_left inst_eq eqs PS.empty. *)
-
-  (* Definition well_structured_memories (eqs: list equation) (M: memories) := *)
-  (*   (forall x, *)
-  (*       find_val x M <> None <-> PS.In x (fbys eqs)) *)
-  (*   /\ forall x, *)
-  (*     find_inst x M <> None <-> PS.In x (insts eqs). *)
-
-  Definition reset_of_value (v: value) : bool :=
+  Definition reset_of (v: value) : bool :=
     match v with
     | present x => x ==b true_val
     | absent => false
     end.
 
-  Definition reset_of (xs: stream value) : stream bool :=
-    fun n => reset_of_value (xs n).
+  (* Definition reset_of (xs: stream value) : stream bool := *)
+  (*   fun n => reset_of_value (xs n). *)
 
-  Definition reset_last (bl: block) (r: stream bool) (x: ident) (xs: stream val) :=
-    fun n =>
-      if r n then
-        match find_init x bl with
-        | Some c => sem_const c
-        | None => false_val
-        end
-      else xs n.
+  Definition reset_last (bl: block) (r: bool) (x: ident) (v: val) : val :=
+    if r then
+      match find_init x bl with
+      | Some c => sem_const c
+      | None => false_val
+      end
+    else v.
 
-  Definition reset_lasts (bl: block) (r: stream bool) (E E0: evolution) :=
-    values E0 = Env.mapi (reset_last bl r) (values E).
+  Definition reset_lasts (bl: block) (r: bool) (S S0: state) : Prop :=
+    values S0 = Env.mapi (reset_last bl r) (values S).
 
-  Section BlockSemantics.
+  Definition same_clock (vs: list value) : Prop :=
+    absent_list vs \/ present_list vs.
+
+  Definition clock_of (vs: list value) (b: bool): Prop :=
+    present_list vs <-> b = true.
+
+  Section Semantics.
 
     Variable P: program.
 
-    Inductive sem_reset: ident -> stream bool -> evolution -> evolution -> Prop :=
+    Inductive sem_reset: ident -> bool -> state -> state -> Prop :=
       SReset:
-        forall b (r: stream bool) E E0 bl P',
+        forall b (r: bool) S S0 bl P',
           find_block b P = Some (bl, P') ->
-          reset_lasts bl r E E0 ->
-          (forall b' E',
-              sub_inst b' E E' ->
-              exists E0',
-                sub_inst b' E0 E0'
-                /\ sem_reset b' r E' E0') ->
-          sem_reset b r E E0.
+          reset_lasts bl r S S0 ->
+          (forall b' S',
+              sub_inst b' S S' ->
+              exists S0',
+                sub_inst b' S0 S0'
+                /\ sem_reset b' r S' S0') ->
+          sem_reset b r S S0.
 
-    Inductive sem_equation: stream bool -> history -> evolution -> transient_evolutions -> evolution -> equation -> Prop :=
+    Inductive sem_equation: bool -> env -> state -> transient_states -> state -> equation -> Prop :=
     | SEqDef:
-        forall bk H E T E' x xs ck ce,
-          sem_var_var H x xs ->
-          sem_caexp bk H E ck ce xs ->
-          sem_equation bk H E T E' (EqDef x ck ce)
+        forall base R S T S' x v ck ce,
+          sem_var_var R x v ->
+          sem_caexp base R S ck ce v ->
+          sem_equation base R S T S' (EqDef x ck ce)
     | SEqNext:
-        forall bk H E T E' x ck e xs ls,
-          sem_state_var bk H E' ck x xs ->
-          sem_laexp bk H E ck e ls ->
-          sem_equation bk H E T E' (EqNext x ck e)
+        forall base R S T S' x ck e v,
+          sem_state_var base R S' ck x v ->
+          sem_laexp base R S ck e v ->
+          sem_equation base R S T S' (EqNext x ck e)
     | SEqTransient:
-        forall bk H E T E' s ck Es,
-          sub_inst s E Es ->
-          PM.find s T = Some Es ->
-          sem_equation bk H E T E' (EqTransient s ck)
+        forall base R S T S' s ck Ss,
+          sub_inst s S Ss ->
+          PM.find s T = Some Ss ->
+          sem_equation base R S T S' (EqTransient s ck)
     | SEqReset:
-        forall bk H E T E' ck b s r rs Es E0,
-          sem_var bk H E ck r rs ->
-          sub_inst s E Es ->
-          sem_reset b (reset_of rs) Es E0 ->
-          PM.find s T = Some E0 ->
-          sem_equation bk H E T E' (EqReset s ck b r)
+        forall base R S T S' ck b s r vr Ss S0,
+          sem_var base R S ck r vr ->
+          sub_inst s S Ss ->
+          sem_reset b (reset_of vr) Ss S0 ->
+          PM.find s T = Some S0 ->
+          sem_equation base R S T S' (EqReset s ck b r)
     | SEqCall:
-        forall bk H E T E' ys ck b s es ess Es oss Es',
-          sem_laexps bk H E ck es ess ->
-          PM.find s T = Some Es ->
-          sem_block b Es ess oss Es' ->
-          sem_vars H ys oss ->
-          sub_inst s E' Es' ->
-          sem_equation bk H E T E' (EqCall s ys ck b es)
+        forall base R S T S' ys ck b s es xs Ss os Ss',
+          sem_laexps base R S ck es xs ->
+          PM.find s T = Some Ss ->
+          sem_block b Ss xs os Ss' ->
+          sem_vars R ys os ->
+          sub_inst s S' Ss' ->
+          sem_equation base R S T S' (EqCall s ys ck b es)
 
-    with sem_block: ident -> evolution -> stream (list value) -> stream (list value) -> evolution -> Prop :=
+    with sem_block: ident -> state -> list value -> list value -> state -> Prop :=
            SBlock:
-             forall b bl P' E T E' H xss yss bk,
-               clock_of xss bk ->
+             forall b bl P' S T S' R xs ys base,
+               clock_of xs base ->
                find_block b P = Some (bl, P') ->
-               sem_vars H (map fst bl.(b_in)) xss ->
-               sem_vars H (map fst bl.(b_out)) yss ->
-               same_clock xss ->
-               same_clock yss ->
-               (forall n, absent_list (xss n) <-> absent_list (yss n)) ->
-               Forall (sem_equation bk H E T E') bl.(b_eqs) ->
+               sem_vars R (map fst bl.(b_in)) xs ->
+               sem_vars R (map fst bl.(b_out)) ys ->
+               same_clock xs ->
+               same_clock ys ->
+               (absent_list xs <-> absent_list ys) ->
+               Forall (sem_equation base R S T S') bl.(b_eqs) ->
                (* well_structured_memories bl.(b_eqs) M -> *)
-               sem_block b E xss yss E'.
+               sem_block b S xs ys S'.
 
-  End BlockSemantics.
+
+  End Semantics.
 
   Section sem_block_mult.
     Variable P: program.
 
-    Variable P_equation: stream bool -> history -> evolution -> transient_evolutions -> evolution -> equation -> Prop.
-    Variable P_block: ident -> evolution -> stream (list value) -> stream (list value) -> evolution -> Prop.
+    Variable P_equation: bool -> env -> state -> transient_states -> state -> equation -> Prop.
+    Variable P_block: ident -> state -> list value -> list value -> state -> Prop.
 
     Hypothesis EqDefCase:
-      forall bk H E T E' x xs ck ce,
-        sem_var_var H x xs ->
-        sem_caexp bk H E ck ce xs ->
-        P_equation bk H E T E' (EqDef x ck ce).
+      forall base R S T S' x v ck ce,
+        sem_var_var R x v ->
+        sem_caexp base R S ck ce v ->
+        P_equation base R S T S' (EqDef x ck ce).
 
     Hypothesis EqNextCase:
-      forall bk H E T E' x ck e xs ls,
-        sem_state_var bk H E' ck x xs ->
-        sem_laexp bk H E ck e ls ->
-        P_equation bk H E T E' (EqNext x ck e).
+      forall base R S T S' x ck e v,
+        sem_state_var base R S' ck x v ->
+        sem_laexp base R S ck e v ->
+        P_equation base R S T S' (EqNext x ck e).
 
     Hypothesis EqTransientCase:
-      forall bk H E T E' s ck Es,
-        sub_inst s E Es ->
-        PM.find s T = Some Es ->
-        P_equation bk H E T E' (EqTransient s ck).
+      forall base R S T S' s ck Ss,
+        sub_inst s S Ss ->
+        PM.find s T = Some Ss ->
+        P_equation base R S T S' (EqTransient s ck).
 
     Hypothesis EqResetCase:
-      forall bk H E T E' ck b s r rs Es E0,
-        sem_var bk H E ck r rs ->
-        sub_inst s E Es ->
-        sem_reset P b (reset_of rs) Es E0 ->
-        PM.find s T = Some E0 ->
-        P_equation bk H E T E' (EqReset s ck b r).
+      forall base R S T S' ck b s r vr Ss S0,
+        sem_var base R S ck r vr ->
+        sub_inst s S Ss ->
+        sem_reset P b (reset_of vr) Ss S0 ->
+        PM.find s T = Some S0 ->
+        P_equation base R S T S' (EqReset s ck b r).
 
     Hypothesis EqCallCase:
-      forall bk H E T E' s ys ck b es ess Es oss Es',
-        sem_laexps bk H E ck es ess ->
-        PM.find s T = Some Es ->
-        sem_block P b Es ess oss Es' ->
-        sem_vars H ys oss ->
-        sub_inst s E' Es' ->
-        P_block b Es ess oss Es' ->
-        P_equation bk H E T E' (EqCall s ys ck b es).
+      forall base R S T S' s ys ck b es xs Ss os Ss',
+        sem_laexps base R S ck es xs ->
+        PM.find s T = Some Ss ->
+        sem_block P b Ss xs os Ss' ->
+        sem_vars R ys os ->
+        sub_inst s S' Ss' ->
+        P_block b Ss xs os Ss' ->
+        P_equation base R S T S' (EqCall s ys ck b es).
 
     Hypothesis BlockCase:
-      forall b bl P' H E T E' xss yss bk,
-        clock_of xss bk ->
+      forall b bl P' R S T S' xs ys base,
+        clock_of xs base ->
         find_block b P = Some (bl, P') ->
-        sem_vars H (map fst bl.(b_in)) xss ->
-        sem_vars H (map fst bl.(b_out)) yss ->
-        same_clock xss ->
-        same_clock yss ->
-        (forall n, absent_list (xss n) <-> absent_list (yss n)) ->
-        Forall (sem_equation P bk H E T E') bl.(b_eqs) ->
-        Forall (P_equation bk H E T E') bl.(b_eqs) ->
-        P_block b E xss yss E'.
+        sem_vars R (map fst bl.(b_in)) xs ->
+        sem_vars R (map fst bl.(b_out)) ys ->
+        same_clock xs ->
+        same_clock ys ->
+        (absent_list xs <-> absent_list ys) ->
+        Forall (sem_equation P base R S T S') bl.(b_eqs) ->
+        Forall (P_equation base R S T S') bl.(b_eqs) ->
+        P_block b S xs ys S'.
 
     Fixpoint sem_equation_mult
-            (b: stream bool) (H: history) (E: evolution) (T: transient_evolutions) (E': evolution) (e: equation)
-            (Sem: sem_equation P b H E T E' e) {struct Sem}
-      : P_equation b H E T E' e
+             (base: bool) (R: env) (S: state) (T: transient_states) (S': state) (e: equation)
+             (Sem: sem_equation P base R S T S' e) {struct Sem}
+      : P_equation base R S T S' e
     with sem_block_mult
-           (f: ident) (E: evolution) (xss oss: stream (list value)) (E': evolution)
-           (Sem: sem_block P f E xss oss E') {struct Sem}
-         : P_block f E xss oss E'.
+           (f: ident) (S: state) (xs ys: list value) (S': state)
+           (Sem: sem_block P f S xs ys S') {struct Sem}
+         : P_block f S xs ys S'.
     Proof.
       - destruct Sem; eauto.
       - destruct Sem.
@@ -605,668 +392,1039 @@ environment.
 
   End sem_block_mult.
 
-  (** Morphisms properties *)
+ (*  (** ** Liftings of instantaneous semantics *) *)
 
-  (* Add Parametric Morphism b A B sem H E : (@lift b H E A B sem) *)
-  (*     with signature eq ==> @eq_str B ==> Basics.impl *)
-  (*       as lift_eq_str. *)
-  (* Proof. *)
-  (*   intros x xs xs' Eq Lift n. *)
-  (*   rewrite <-Eq; auto. *)
-  (* Qed. *)
+(*   Section LiftSemantics. *)
 
-  (* Add Parametric Morphism A B sem H E : (@lift' H E A B sem) *)
-  (*     with signature eq ==> @eq_str B ==> Basics.impl *)
-  (*       as lift'_eq_str. *)
-  (* Proof. *)
-  (*   intros x xs xs' Eq Lift n. *)
-  (*   rewrite <-Eq; auto. *)
-  (* Qed. *)
-
-  (* Add Parametric Morphism A B sem E : (@lift'' E A B sem) *)
-  (*     with signature eq ==> @eq_str B ==> Basics.impl *)
-  (*       as lift''_eq_str. *)
-  (* Proof. *)
-  (*   intros x xs xs' Eq Lift n. *)
-  (*   rewrite <-Eq; auto. *)
-  (* Qed. *)
-
-  (* Add Parametric Morphism A B sem H : (@lift''' H A B sem) *)
-  (*     with signature eq ==> @eq_str B ==> Basics.impl *)
-  (*       as lift'''_eq_str. *)
-  (* Proof. *)
-  (*   intros x xs xs' Eq Lift n. *)
-  (*   rewrite <-Eq; auto. *)
-  (* Qed. *)
-
-  (* Add Parametric Morphism : clock_of *)
-  (*     with signature eq_str ==> eq ==> Basics.impl *)
-  (*       as clock_of_eq_str. *)
-  (* Proof. *)
-  (*   unfold clock_of. intros ** E b Pres n. *)
-  (*   split; intros H. *)
-  (*   - apply Pres. *)
-  (*     specialize (E n). *)
-  (*     induction H; rewrite E; constructor; auto. *)
-  (*   - apply Pres in H. *)
-  (*     specialize (E n). *)
-  (*     induction H; rewrite <-E; constructor; auto. *)
-  (* Qed. *)
-
-  (* Add Parametric Morphism : reset_of *)
-  (*     with signature eq_str ==> eq_str *)
-  (*       as reset_of_eq_str. *)
-  (* Proof. *)
-  (*   unfold reset_of. intros ** E n. *)
-  (*   now rewrite E. *)
-  (* Qed. *)
-
-  (* Add Parametric Morphism : reset_regs *)
-  (*     with signature eq_str ==> eq ==> Basics.impl *)
-  (*       as reset_regs_eq_str. *)
-  (* Proof. *)
-  (*   intros ** E M Rst. *)
-  (*   induction Rst; constructor; eauto. *)
-  (* Qed. *)
-
-  Add Parametric Morphism : same_clock
-      with signature eq_str ==> Basics.impl
-        as same_clock_eq_str.
-  Proof.
-    unfold same_clock; intros ** E ? ?; rewrite <-E; auto.
-  Qed.
-
-  (** ** Clocking property *)
-
-  Lemma not_subrate_clock:
-    forall R S ck,
-      ~ sem_clock_instant false R S ck true.
-  Proof.
-    intros ** Sem; induction ck; inv Sem.
-    now apply IHck.
-  Qed.
-
-  Lemma present_not_absent_list:
-    forall xs (vs: list val),
-      instant_same_clock xs ->
-      ~ absent_list xs ->
-      present_list xs.
-  Proof.
-    intros ** Hsamexs Hnabs.
-    now destruct Hsamexs.
-  Qed.
-
-  Lemma sem_vars_gt0:
-    forall H (xs: list (ident * type)) ls,
-      0 < length xs ->
-      sem_vars H (map fst xs) ls ->
-      forall n, 0 < length (ls n).
-  Proof.
-    intros ** Hgt0 Hsem n.
-    specialize (Hsem n).
-    apply Forall2_length in Hsem.
-    rewrite map_length in Hsem.
-    now rewrite Hsem in Hgt0.
-  Qed.
-
-  Ltac assert_const_length xss :=
-    match goal with
-      H: sem_vars _ _ xss |- _ =>
-      let H' := fresh in
-      let k := fresh in
-      let k' := fresh in
-      assert (wf_streams xss)
-        by (intros k k'; pose proof H as H';
-            unfold sem_vars, lift in *;
-            specialize (H k); specialize (H' k');
-            apply Forall2_length in H; apply Forall2_length in H';
-            now rewrite H in H')
-    end.
-
-  (** ** Determinism of the semantics *)
-
-  (** *** Instantaneous semantics *)
-
-  Section InstantDeterminism.
-
-    Variable base: bool.
-    Variable R: env.
-    Variable S: state.
-
-    Lemma sem_var_var_instant_det:
-      forall x v1 v2,
-        sem_var_var_instant R x v1
-        -> sem_var_var_instant R x v2
-        -> v1 = v2.
-    Proof.
-      intros x v1 v2 H1 H2.
-      inversion_clear H1 as [Hf1];
-        inversion_clear H2 as [Hf2];
-        congruence.
-    Qed.
-    Hint Resolve sem_var_var_instant_det.
-
-    Lemma sem_clock_state_var_var_instant_det:
-      (forall ck v1,
-          sem_clock_instant base R S ck v1 ->
-          forall v2,
-            sem_clock_instant base R S ck v2 ->
-            v1 = v2)
-      /\
-      (forall ck x v1,
-          sem_state_var_instant base R S ck x v1 ->
-          forall v2,
-            sem_state_var_instant base R S ck x v2 ->
-            v1 = v2)
-      /\
-      (forall ck x v1,
-          sem_var_instant base R S ck x v1 ->
-          forall v2,
-            sem_var_instant base R S ck x v2 ->
-            v1 = v2).
-    Proof.
-      apply sem_clock_state_var_var_mut.
-      - intro; now inversion 1.
-      - intros ** VarDet ?? Sem.
-        inversion Sem as [ | | |??? b' ? SVar]; subst; auto.
-        apply VarDet in SVar; inv SVar.
-        destruct b'; simpl in *; congruence.
-      - intros ** Sem; inv Sem; auto.
-      - intros ** VarDet ?? Sem.
-        inversion Sem as [ |????? SVar| |]; subst; auto.
-        apply VarDet in SVar; inv SVar.
-        destruct b; simpl in *; congruence.
-      - intros ** ClockDet ? Sem.
-        inversion_clear Sem as [|??? SClock]; try congruence.
-        apply ClockDet in SClock; discriminate.
-      - intros ** ClockDet ? Sem.
-        inversion_clear Sem as [???? SClock|]; auto.
-        apply ClockDet in SClock; discriminate.
-      - intros ** Sem; inv Sem; eauto.
-      - intros ** Sem; inv Sem; auto.
-    Qed.
-
-    Corollary sem_clock_instant_det:
-      forall ck v1 v2,
-        sem_clock_instant base R S ck v1
-        -> sem_clock_instant base R S ck v2
-        -> v1 = v2.
-    Proof.
-      intros; eapply sem_clock_state_var_var_instant_det; eauto.
-    Qed.
-    Hint Resolve sem_clock_instant_det.
-
-    Corollary sem_state_var_instant_det:
-      forall x ck v1 v2,
-        sem_state_var_instant base R S ck x v1
-        -> sem_state_var_instant base R S ck x v2
-        -> v1 = v2.
-    Proof.
-      intros; eapply (proj1 (proj2 sem_clock_state_var_var_instant_det)); eauto.
-    Qed.
-    Hint Resolve sem_state_var_instant_det.
-
-    Corollary sem_var_instant_det:
-      forall x ck v1 v2,
-        sem_var_instant base R S ck x v1
-        -> sem_var_instant base R S ck x v2
-        -> v1 = v2.
-    Proof.
-      intros; eapply sem_clock_state_var_var_instant_det; eauto.
-    Qed.
-    Hint Resolve sem_var_instant_det.
-
-    Lemma sem_lexp_instant_det:
-      forall e ck v1 v2,
-        sem_lexp_instant base R S ck e v1
-        -> sem_lexp_instant base R S ck e v2
-        -> v1 = v2.
-    Proof.
-      induction e (* using lexp_ind2 *).
-      - (* Econst *)
-        do 2 inversion_clear 1; destruct base; congruence.
-      - (* Evar *)
-        intros ** S1 S2; inv S1; inv S2; eauto.
-      - (* Ewhen *)
-        intros ** S1 S2; inv S1; inv S2; eauto;
-          repeat progress match goal with
-                          | H1:sem_lexp_instant ?b ?R ?S ?ck ?e ?v1,
-                               H2:sem_lexp_instant ?b ?R ?S ?ck ?e ?v2 |- _ =>
-                            apply IHe with (1:=H1) in H2
-                          | H1:sem_var_instant ?b ?R ?S ?ck ?i ?v1,
-                               H2:sem_var_instant ?b ?R ?S ?ck ?i ?v2 |- _ =>
-                            apply sem_var_instant_det with (1:=H1) in H2
-                          | Hp:present _ = present _ |- _ =>
-                            injection Hp; intro; subst
-                          | H1:val_to_bool _ = Some _,
-                               H2:val_to_bool _ = Some (negb _) |- _ =>
-                            rewrite H2 in H1; exfalso; injection H1;
-                              now apply Bool.no_fixpoint_negb
-                          end; subst; auto.
-      - (* Eunop *)
-        intros ** S1 S2; inv S1; inv S2;
-          repeat progress match goal with
-                          | H1:sem_lexp_instant _ _ _ _ e _, H2:sem_lexp_instant _ _ _ _ e _ |- _ =>
-                            apply IHe with (1:=H1) in H2; inversion H2; subst
-                          | H1:sem_unop _ _ _ = _, H2:sem_unop _ _ _ = _ |- _ =>
-                            rewrite H1 in H2; injection H2; intro; subst
-                          | H1:sem_lexp_instant _ _ _ _ _ (present _),
-                               H2:sem_lexp_instant _ _ _ _ _ absent |- _ =>
-                            apply IHe with (1:=H1) in H2
-                          end; try auto.
-      - (* Ebinop *)
-        intros ** S1 S2; inv S1; inv S2;
-          repeat progress match goal with
-                          | H1:sem_lexp_instant _ _ _ _ e1 _, H2:sem_lexp_instant _ _ _ _ e1 _ |- _ =>
-                            apply IHe1 with (1:=H1) in H2
-                          | H1:sem_lexp_instant _ _ _ _ e2 _, H2:sem_lexp_instant _ _ _ _ e2 _ |- _ =>
-                            apply IHe2 with (1:=H1) in H2
-                          | H1:sem_binop _ _ _ _ _ = Some ?v1,
-                               H2:sem_binop _ _ _ _ _ = Some ?v2 |- _ =>
-                            rewrite H1 in H2; injection H2; intro; subst
-                          | H:present _ = present _ |- _ => injection H; intro; subst
-                          end; subst; auto; discriminate.
-    Qed.
-    Hint Resolve sem_lexp_instant_det.
-
-    Lemma sem_laexp_instant_det:
-      forall ck e v1 v2,
-        sem_laexp_instant base R S ck e v1
-        -> sem_laexp_instant base R S ck e v2
-        -> v1 = v2.
-    Proof.
-      do 2 inversion_clear 1; eauto.
-    Qed.
-
-    Lemma sem_lexps_instant_det:
-      forall les ck cs1 cs2,
-        sem_lexps_instant base R S ck les cs1 ->
-        sem_lexps_instant base R S ck les cs2 ->
-        cs1 = cs2.
-    Proof.
-      intros ???; eapply Forall2_det; eauto.
-    Qed.
-    Hint Resolve sem_lexps_instant_det.
-
-    Lemma sem_laexps_instant_det:
-      forall ck e v1 v2,
-        sem_laexps_instant base R S ck e v1
-        -> sem_laexps_instant base R S ck e v2
-        -> v1 = v2.
-    Proof.
-      do 2 inversion_clear 1; eauto.
-    Qed.
-
-    Lemma sem_cexp_instant_det:
-      forall e ck v1 v2,
-        sem_cexp_instant base R S ck e v1
-        -> sem_cexp_instant base R S ck e v2
-        -> v1 = v2.
-    Proof.
-      induction e;
-        do 2 inversion_clear 1;
-        try repeat progress match goal with
-                            | H1: sem_cexp_instant ?bk ?R ?S ?ck ?e ?l,
-                                  H2: sem_cexp_instant ?bk ?R ?S ?ck ?e ?r |- _ =>
-                              apply IHe1 with (1:=H1) in H2
-                                                         || apply IHe2 with (1:=H1) in H2;
-                                injection H2; intro; subst
-                            | H1: sem_var_instant ?b ?R ?S ?ck ?i (present true_val),
-                                  H2: sem_var_instant ?b ?R ?S ?ck ?i (present false_val) |- _ =>
-                              apply sem_var_instant_det with (1:=H1) in H2;
-                                exfalso; injection H2; now apply true_not_false_val
-                            | H1: sem_lexp_instant ?bk ?R ?S ?ck ?l ?v1,
-                                  H2: sem_lexp_instant ?bk ?R ?S ?ck ?l ?v2 |- _ =>
-                              apply sem_lexp_instant_det with (1:=H1) in H2;
-                                discriminate || injection H2; intro; subst
-                            | H1: sem_var_instant ?bk ?R ?S ?ck ?i (present _),
-                                  H2: sem_var_instant ?bk ?R ?S ?ck ?i absent |- _ =>
-                              apply sem_var_instant_det with (1:=H1) in H2; discriminate
-                            | H1: val_to_bool _ = Some _,
-                                  H2:val_to_bool _ = Some _ |- _ =>
-                              rewrite H1 in H2; injection H2; intro; subst
-                            end; eauto.
-    Qed.
-    Hint Resolve sem_cexp_instant_det.
-
-    Lemma sem_caexp_instant_det:
-      forall ck e v1 v2,
-        sem_caexp_instant base R S ck e v1
-        -> sem_caexp_instant base R S ck e v2
-        -> v1 = v2.
-    Proof.
-      intros until v2.
-      do 2 inversion_clear 1; eauto.
-    Qed.
-
-  End InstantDeterminism.
-
-  (** *** Lifted semantics *)
-
-  (* Section LiftDeterminism. *)
-
-(*     Variable bk : stream bool. *)
+(*     Variable base : stream bool. *)
 (*     Variable H : history. *)
+(*     Variable E : evolution. *)
 
-(*     Require Import Logic.FunctionalExtensionality. *)
+(*     Definition sample {A} (n: nat) (xs: stream A) := xs n. *)
+(*     Hint Unfold sample. *)
 
-(*     Lemma lift_det: *)
-(*       forall {A B} (P: bool -> env -> A -> B -> Prop) (bk: stream bool) *)
-(*         x (xs1 xs2 : stream B), *)
-(*         (forall b R v1 v2, P b R x v1 -> P b R x v2 -> v1 = v2) -> *)
-(*         lift bk H P x xs1 -> lift bk H P x xs2 -> xs1 = xs2. *)
+(*     Definition restr_evol (n: nat): state := *)
+(*       mmap (sample n) E. *)
+
+(*     Definition restr_hist (n: nat): env := *)
+(*       PM.map (sample n) H. *)
+(*     Hint Unfold restr_hist. *)
+
+(*     Definition lift {A B} (sem: bool -> env -> state -> clock -> A -> B -> Prop) *)
+(*                ck x (ys: stream B): Prop := *)
+(*       forall n, sem (bk n) (restr_hist n) (restr_evol n) ck x (ys n). *)
+(*     Hint Unfold lift. *)
+
+(*     Definition lift' {A B} (sem: env -> state -> clock -> A -> B -> Prop) ck x (ys: stream B): Prop := *)
+(*       forall n, sem (restr_hist n) (restr_evol n) ck x (ys n). *)
+(*     Hint Unfold lift'. *)
+
+(*     Definition lift'' {A B} (sem: env -> clock -> A -> B -> Prop) ck x (ys: stream B): Prop := *)
+(*       forall n, sem (restr_hist n) ck x (ys n). *)
+(*     Hint Unfold lift''. *)
+
+(*     Definition lift''' {A B} (sem: state -> clock -> A -> B -> Prop) ck x (ys: stream B): Prop := *)
+(*       forall n, sem (restr_evol n) ck x (ys n). *)
+(*     Hint Unfold lift'''. *)
+
+(*     Definition lift'''' {A B} (sem: bool -> env -> state -> A -> B -> Prop) *)
+(*                x (ys: stream B): Prop := *)
+(*       forall n, sem (bk n) (restr_hist n) (restr_evol n) x (ys n). *)
+(*     Hint Unfold lift''''. *)
+
+(*     Definition lift''''' {A B} (sem: env -> A -> B -> Prop) *)
+(*                x (ys: stream B): Prop := *)
+(*       forall n, sem (restr_hist n) x (ys n). *)
+(*     Hint Unfold lift'''''. *)
+(*     (* Definition lift''' {A B} (sem: bool -> env -> A -> B -> Prop) x (ys: stream B): Prop := *) *)
+(*     (*   forall n, sem (bk n) (restr_hist n) x (ys n). *) *)
+(*     (* Hint Unfold lift'''. *) *)
+
+(*     Definition sem_clock (ck: clock) (xs: stream bool): Prop := *)
+(*       lift'''' sem_clock ck xs. *)
+
+(*     Definition sem_var ck (x: var) (xs: stream value): Prop := *)
+(*       lift sem_var ck x xs. *)
+
+(*     (* Definition sem_last (x: ident) (xs: stream value): Prop := *) *)
+(*     (*   lift'' sem_last x xs. *) *)
+
+(*     Definition sem_var_var (x: ident) (xs: stream value): Prop := *)
+(*       lift''''' sem_var_var x xs. *)
+
+(*     Definition sem_state_var ck (x: ident) (xs: stream value): Prop := *)
+(*       lift sem_state_var ck x xs. *)
+
+(*     Definition sem_vars (x: idents) (xs: stream (list value)): Prop := *)
+(*       lift''''' sem_vars x xs. *)
+
+(*     Definition sem_laexp ck (e: lexp) (xs: stream value): Prop := *)
+(*       lift'''' (fun base R S => sem_laexp base R S ck) e xs. *)
+
+(*     Definition sem_laexps (ck: clock) (e: list lexp) (xs: stream (list value)): Prop := *)
+(*       lift'''' (fun base R S => sem_laexps base R S ck) e xs. *)
+
+(*     Definition sem_lexp ck (e: lexp) (xs: stream value): Prop := *)
+(*       lift sem_lexp ck e xs. *)
+
+(*     Definition sem_lexps ck (e: list lexp) (xs: stream (list value)): Prop := *)
+(*       lift sem_lexps ck e xs. *)
+
+(*     Definition sem_caexp ck (c: cexp) (xs: stream value): Prop := *)
+(*       lift'''' (fun base R S => sem_caexp base R S ck) c xs. *)
+
+(*     Definition sem_cexp ck (c: cexp) (xs: stream value): Prop := *)
+(*       lift sem_cexp ck c xs. *)
+
+(*   End LiftSemantics. *)
+
+(*   (** ** Time-dependent semantics *) *)
+
+(*   Definition instant_same_clock (l : list value) : Prop := *)
+(*     absent_list l \/ present_list l. *)
+
+(*   Definition same_clock (l_s : stream (list value)) : Prop := *)
+(*     forall n, instant_same_clock (l_s n). *)
+
+(*   Definition clock_of (xss: stream (list value))(bs: stream bool): Prop := *)
+(*     forall n, *)
+(*       present_list (xss n) <-> bs n = true. *)
+
+(*   Definition clock_of' (xss: stream (list value)) : stream bool := *)
+(*     fun n => forallb (fun v => negb (v ==b absent)) (xss n). *)
+
+(*   Lemma clock_of_equiv: *)
+(*     forall xss, clock_of xss (clock_of' xss). *)
+(*   Proof. *)
+(*     split; intros H. *)
+(*     - unfold clock_of'. *)
+(*       rewrite forallb_forall. *)
+(*       intros; rewrite Bool.negb_true_iff. *)
+(*       rewrite not_equiv_decb_equiv. *)
+(*       eapply In_Forall in H; eauto. *)
+(*     - unfold clock_of' in H. *)
+(*       rewrite forallb_forall in H. *)
+(*       apply all_In_Forall; intros ** Hin E. *)
+(*       specialize (H _ Hin). *)
+(*       rewrite Bool.negb_true_iff, not_equiv_decb_equiv in H. *)
+(*       apply H; eauto. *)
+(*   Qed. *)
+
+(*   Lemma clock_of_equiv': *)
+(*     forall xss bk, *)
+(*       clock_of xss bk -> *)
+(*       bk ≈ clock_of' xss. *)
+(*   Proof. *)
+(*     intros ** H n; specialize (H n). *)
+(*     unfold clock_of'. *)
+(*     induction (xss n) as [|v]; simpl. *)
+(*     - apply H; constructor. *)
+(*     - destruct v. *)
+(*       + simpl. *)
+(*         rewrite <-Bool.not_true_iff_false, <-H. *)
+(*         inversion 1; auto. *)
+(*       + simpl. *)
+(*         apply IHl; rewrite <-H. *)
+(*         split; intro P. *)
+(*         * constructor; auto. *)
+(*           intro; discriminate. *)
+(*         * inv P; auto. *)
+(*   Qed. *)
+
+(*   (* Record mvalues := *) *)
+(*   (*   Mvalues { content: stream val; *) *)
+(*   (*             reset: stream bool *) *)
+(*   (*           }. *) *)
+
+(*   (* (* Definition memory := RMemory.memory mvalue. *) *) *)
+(*   (* Definition memories := RMemory.memory mvalues. *) *)
+
+(*   (* Inductive reset_regs: stream bool -> memories -> Prop := *) *)
+(*   (*   reset_regs_intro: *) *)
+(*   (*     forall M rs, *) *)
+(*   (*       (forall x mvs, *) *)
+(*   (*           find_val x M = Some mvs -> *) *)
+(*   (*           forall n, rs n = true -> mvs.(reset) n = true) -> *) *)
+(*   (*       (forall x M', *) *)
+(*   (*           sub_inst x M M' -> *) *)
+(*   (*           reset_regs rs M') -> *) *)
+(*   (*       reset_regs rs M. *) *)
+
+(*   (* (* Definition next (n: nat) (mvs: mvalues) (v0 v: val) : Prop := *) *) *)
+(*   (* (*   mvs.(content) (S n) = (if mvs.(reset) (S n) then v0 else v). *) *) *)
+
+(*   (* (* Inductive fby_spec: nat -> val -> value -> mvalues -> value -> Prop := *) *) *)
+(*   (* (* | fby_spec_present: *) *) *)
+(*   (* (*     forall n v0 v mvs, *) *) *)
+(*   (* (*       next n mvs v0 v -> *) *) *)
+(*   (* (*       fby_spec n v0 (present v) mv (mv.(content) n) *) *) *)
+(*   (* (* | fby_spec_absent: *) *) *)
+(*   (* (*     forall n v0 v mvs, *) *) *)
+(*   (* (*       next n mvs v0 (mvs.(content) n) -> *) *) *)
+(*   (* (*       fby_spec n v0 absent mvs absent. *) *) *)
+
+(*   (* Inductive mfby: ident -> val -> stream value -> memories -> stream value -> Prop := *) *)
+(*   (*   mfby_intro: *) *)
+(*   (*     forall x mvs v0 ls M xs, *) *)
+(*   (*       find_val x M = Some mvs -> *) *)
+(*   (*       mvs.(content) 0 = v0 -> *) *)
+(*   (*       (forall n, match ls n with *) *)
+(*   (*             | absent => *) *)
+(*   (*               mvs.(content) (S n) = (if mvs.(reset) (S n) then v0 else mvs.(content) n) *) *)
+(*   (*               /\ xs n = absent *) *)
+(*   (*             | present v => *) *)
+(*   (*               mvs.(content) (S n) = (if mvs.(reset) (S n) then v0 else v) *) *)
+(*   (*               /\ xs n = present (mvs.(content) n) *) *)
+(*   (*             end) -> *) *)
+(*   (*       mfby x v0 ls M xs. *) *)
+
+(*   (* Definition fby_eq (mems: PS.t) (eq: equation) : PS.t := *) *)
+(*   (*   match eq with *) *)
+(*   (*   | EqFby x _ _ _ => PS.add x mems *) *)
+(*   (*   | _ => mems *) *)
+(*   (*   end. *) *)
+
+(*   (* Definition fbys (eqs: list equation) : PS.t := *) *)
+(*   (*   fold_left fby_eq eqs PS.empty. *) *)
+
+(*   (* Definition inst_eq (insts: PS.t) (eq: equation) : PS.t := *) *)
+(*   (*   match eq with *) *)
+(*   (*   | EqReset _ _ i _ => PS.add i insts *) *)
+(*   (*   | EqCall _ _ _ i _ => PS.add i insts *) *)
+(*   (*   | _ => insts *) *)
+(*   (*   end. *) *)
+
+(*   (* Definition insts (eqs: list equation) : PS.t := *) *)
+(*   (*   fold_left inst_eq eqs PS.empty. *) *)
+
+(*   (* Definition well_structured_memories (eqs: list equation) (M: memories) := *) *)
+(*   (*   (forall x, *) *)
+(*   (*       find_val x M <> None <-> PS.In x (fbys eqs)) *) *)
+(*   (*   /\ forall x, *) *)
+(*   (*     find_inst x M <> None <-> PS.In x (insts eqs). *) *)
+
+(*   Definition reset_of_value (v: value) : bool := *)
+(*     match v with *)
+(*     | present x => x ==b true_val *)
+(*     | absent => false *)
+(*     end. *)
+
+(*   Definition reset_of (xs: stream value) : stream bool := *)
+(*     fun n => reset_of_value (xs n). *)
+
+(*   Definition reset_last (bl: block) (r: stream bool) (x: ident) (xs: stream val) := *)
+(*     fun n => *)
+(*       if r n then *)
+(*         match find_init x bl with *)
+(*         | Some c => sem_const c *)
+(*         | None => false_val *)
+(*         end *)
+(*       else xs n. *)
+
+(*   Definition reset_lasts (bl: block) (r: stream bool) (E E0: evolution) := *)
+(*     values E0 = Env.mapi (reset_last bl r) (values E). *)
+
+(*   Section BlockSemantics. *)
+
+(*     Variable P: program. *)
+
+(*     Inductive sem_reset: ident -> stream bool -> evolution -> evolution -> Prop := *)
+(*       SReset: *)
+(*         forall b (r: stream bool) E E0 bl P', *)
+(*           find_block b P = Some (bl, P') -> *)
+(*           reset_lasts bl r E E0 -> *)
+(*           (forall b' E', *)
+(*               sub_inst b' E E' -> *)
+(*               exists E0', *)
+(*                 sub_inst b' E0 E0' *)
+(*                 /\ sem_reset b' r E' E0') -> *)
+(*           sem_reset b r E E0. *)
+
+(*     Inductive sem_equation: stream bool -> history -> evolution -> transient_evolutions -> evolution -> equation -> Prop := *)
+(*     | SEqDef: *)
+(*         forall bk H E T E' x xs ck ce, *)
+(*           sem_var_var H x xs -> *)
+(*           sem_caexp bk H E ck ce xs -> *)
+(*           sem_equation bk H E T E' (EqDef x ck ce) *)
+(*     | SEqNext: *)
+(*         forall bk H E T E' x ck e xs ls, *)
+(*           sem_state_var bk H E' ck x xs -> *)
+(*           sem_laexp bk H E ck e ls -> *)
+(*           sem_equation bk H E T E' (EqNext x ck e) *)
+(*     | SEqTransient: *)
+(*         forall bk H E T E' s ck Es, *)
+(*           sub_inst s E Es -> *)
+(*           PM.find s T = Some Es -> *)
+(*           sem_equation bk H E T E' (EqTransient s ck) *)
+(*     | SEqReset: *)
+(*         forall bk H E T E' ck b s r rs Es E0, *)
+(*           sem_var bk H E ck r rs -> *)
+(*           sub_inst s E Es -> *)
+(*           sem_reset b (reset_of rs) Es E0 -> *)
+(*           PM.find s T = Some E0 -> *)
+(*           sem_equation bk H E T E' (EqReset s ck b r) *)
+(*     | SEqCall: *)
+(*         forall bk H E T E' ys ck b s es ess Es oss Es', *)
+(*           sem_laexps bk H E ck es ess -> *)
+(*           PM.find s T = Some Es -> *)
+(*           sem_block b Es ess oss Es' -> *)
+(*           sem_vars H ys oss -> *)
+(*           sub_inst s E' Es' -> *)
+(*           sem_equation bk H E T E' (EqCall s ys ck b es) *)
+
+(*     with sem_block: ident -> evolution -> stream (list value) -> stream (list value) -> evolution -> Prop := *)
+(*            SBlock: *)
+(*              forall b bl P' E T E' H xss yss bk, *)
+(*                clock_of xss bk -> *)
+(*                find_block b P = Some (bl, P') -> *)
+(*                sem_vars H (map fst bl.(b_in)) xss -> *)
+(*                sem_vars H (map fst bl.(b_out)) yss -> *)
+(*                same_clock xss -> *)
+(*                same_clock yss -> *)
+(*                (forall n, absent_list (xss n) <-> absent_list (yss n)) -> *)
+(*                Forall (sem_equation bk H E T E') bl.(b_eqs) -> *)
+(*                (* well_structured_memories bl.(b_eqs) M -> *) *)
+(*                sem_block b E xss yss E'. *)
+
+(*   End BlockSemantics. *)
+
+(*   Section sem_block_mult. *)
+(*     Variable P: program. *)
+
+(*     Variable P_equation: stream bool -> history -> evolution -> transient_evolutions -> evolution -> equation -> Prop. *)
+(*     Variable P_block: ident -> evolution -> stream (list value) -> stream (list value) -> evolution -> Prop. *)
+
+(*     Hypothesis EqDefCase: *)
+(*       forall bk H E T E' x xs ck ce, *)
+(*         sem_var_var H x xs -> *)
+(*         sem_caexp bk H E ck ce xs -> *)
+(*         P_equation bk H E T E' (EqDef x ck ce). *)
+
+(*     Hypothesis EqNextCase: *)
+(*       forall bk H E T E' x ck e xs ls, *)
+(*         sem_state_var bk H E' ck x xs -> *)
+(*         sem_laexp bk H E ck e ls -> *)
+(*         P_equation bk H E T E' (EqNext x ck e). *)
+
+(*     Hypothesis EqTransientCase: *)
+(*       forall bk H E T E' s ck Es, *)
+(*         sub_inst s E Es -> *)
+(*         PM.find s T = Some Es -> *)
+(*         P_equation bk H E T E' (EqTransient s ck). *)
+
+(*     Hypothesis EqResetCase: *)
+(*       forall bk H E T E' ck b s r rs Es E0, *)
+(*         sem_var bk H E ck r rs -> *)
+(*         sub_inst s E Es -> *)
+(*         sem_reset P b (reset_of rs) Es E0 -> *)
+(*         PM.find s T = Some E0 -> *)
+(*         P_equation bk H E T E' (EqReset s ck b r). *)
+
+(*     Hypothesis EqCallCase: *)
+(*       forall bk H E T E' s ys ck b es ess Es oss Es', *)
+(*         sem_laexps bk H E ck es ess -> *)
+(*         PM.find s T = Some Es -> *)
+(*         sem_block P b Es ess oss Es' -> *)
+(*         sem_vars H ys oss -> *)
+(*         sub_inst s E' Es' -> *)
+(*         P_block b Es ess oss Es' -> *)
+(*         P_equation bk H E T E' (EqCall s ys ck b es). *)
+
+(*     Hypothesis BlockCase: *)
+(*       forall b bl P' H E T E' xss yss bk, *)
+(*         clock_of xss bk -> *)
+(*         find_block b P = Some (bl, P') -> *)
+(*         sem_vars H (map fst bl.(b_in)) xss -> *)
+(*         sem_vars H (map fst bl.(b_out)) yss -> *)
+(*         same_clock xss -> *)
+(*         same_clock yss -> *)
+(*         (forall n, absent_list (xss n) <-> absent_list (yss n)) -> *)
+(*         Forall (sem_equation P bk H E T E') bl.(b_eqs) -> *)
+(*         Forall (P_equation bk H E T E') bl.(b_eqs) -> *)
+(*         P_block b E xss yss E'. *)
+
+(*     Fixpoint sem_equation_mult *)
+(*             (b: stream bool) (H: history) (E: evolution) (T: transient_evolutions) (E': evolution) (e: equation) *)
+(*             (Sem: sem_equation P b H E T E' e) {struct Sem} *)
+(*       : P_equation b H E T E' e *)
+(*     with sem_block_mult *)
+(*            (f: ident) (E: evolution) (xss oss: stream (list value)) (E': evolution) *)
+(*            (Sem: sem_block P f E xss oss E') {struct Sem} *)
+(*          : P_block f E xss oss E'. *)
 (*     Proof. *)
-(*       intros ** Hpoint H1 H2. *)
-(*       extensionality n. specialize (H1 n). specialize (H2 n). *)
-(*       eapply Hpoint; eassumption. *)
+(*       - destruct Sem; eauto. *)
+(*       - destruct Sem. *)
+(*         eapply BlockCase; eauto. *)
+(*         match goal with H: Forall _ _ |- _ => induction H; auto end. *)
 (*     Qed. *)
 
-(*     Lemma lift'_det: *)
-(*       forall {A B} (P: env -> A -> B -> Prop) *)
-(*         x (xs1 xs2 : stream B), *)
-(*         (forall R v1 v2, P R x v1 -> P R x v2 -> v1 = v2) -> *)
-(*         lift' H P x xs1 -> lift' H P x xs2 -> xs1 = xs2. *)
+(*     Combined Scheme sem_equation_block_ind from *)
+(*              sem_equation_mult, sem_block_mult. *)
+
+(*   End sem_block_mult. *)
+
+(*   (** Morphisms properties *) *)
+
+(*   (* Add Parametric Morphism b A B sem H E : (@lift b H E A B sem) *) *)
+(*   (*     with signature eq ==> @eq_str B ==> Basics.impl *) *)
+(*   (*       as lift_eq_str. *) *)
+(*   (* Proof. *) *)
+(*   (*   intros x xs xs' Eq Lift n. *) *)
+(*   (*   rewrite <-Eq; auto. *) *)
+(*   (* Qed. *) *)
+
+(*   (* Add Parametric Morphism A B sem H E : (@lift' H E A B sem) *) *)
+(*   (*     with signature eq ==> @eq_str B ==> Basics.impl *) *)
+(*   (*       as lift'_eq_str. *) *)
+(*   (* Proof. *) *)
+(*   (*   intros x xs xs' Eq Lift n. *) *)
+(*   (*   rewrite <-Eq; auto. *) *)
+(*   (* Qed. *) *)
+
+(*   (* Add Parametric Morphism A B sem E : (@lift'' E A B sem) *) *)
+(*   (*     with signature eq ==> @eq_str B ==> Basics.impl *) *)
+(*   (*       as lift''_eq_str. *) *)
+(*   (* Proof. *) *)
+(*   (*   intros x xs xs' Eq Lift n. *) *)
+(*   (*   rewrite <-Eq; auto. *) *)
+(*   (* Qed. *) *)
+
+(*   (* Add Parametric Morphism A B sem H : (@lift''' H A B sem) *) *)
+(*   (*     with signature eq ==> @eq_str B ==> Basics.impl *) *)
+(*   (*       as lift'''_eq_str. *) *)
+(*   (* Proof. *) *)
+(*   (*   intros x xs xs' Eq Lift n. *) *)
+(*   (*   rewrite <-Eq; auto. *) *)
+(*   (* Qed. *) *)
+
+(*   (* Add Parametric Morphism : clock_of *) *)
+(*   (*     with signature eq_str ==> eq ==> Basics.impl *) *)
+(*   (*       as clock_of_eq_str. *) *)
+(*   (* Proof. *) *)
+(*   (*   unfold clock_of. intros ** E b Pres n. *) *)
+(*   (*   split; intros H. *) *)
+(*   (*   - apply Pres. *) *)
+(*   (*     specialize (E n). *) *)
+(*   (*     induction H; rewrite E; constructor; auto. *) *)
+(*   (*   - apply Pres in H. *) *)
+(*   (*     specialize (E n). *) *)
+(*   (*     induction H; rewrite <-E; constructor; auto. *) *)
+(*   (* Qed. *) *)
+
+(*   (* Add Parametric Morphism : reset_of *) *)
+(*   (*     with signature eq_str ==> eq_str *) *)
+(*   (*       as reset_of_eq_str. *) *)
+(*   (* Proof. *) *)
+(*   (*   unfold reset_of. intros ** E n. *) *)
+(*   (*   now rewrite E. *) *)
+(*   (* Qed. *) *)
+
+(*   (* Add Parametric Morphism : reset_regs *) *)
+(*   (*     with signature eq_str ==> eq ==> Basics.impl *) *)
+(*   (*       as reset_regs_eq_str. *) *)
+(*   (* Proof. *) *)
+(*   (*   intros ** E M Rst. *) *)
+(*   (*   induction Rst; constructor; eauto. *) *)
+(*   (* Qed. *) *)
+
+(*   Add Parametric Morphism : same_clock *)
+(*       with signature eq_str ==> Basics.impl *)
+(*         as same_clock_eq_str. *)
+(*   Proof. *)
+(*     unfold same_clock; intros ** E ? ?; rewrite <-E; auto. *)
+(*   Qed. *)
+
+(*   (** ** Clocking property *) *)
+
+(*   Lemma not_subrate_clock: *)
+(*     forall R S ck, *)
+(*       ~ sem_clock_instant false R S ck true. *)
+(*   Proof. *)
+(*     intros ** Sem; induction ck; inv Sem. *)
+(*     now apply IHck. *)
+(*   Qed. *)
+
+(*   Lemma present_not_absent_list: *)
+(*     forall xs (vs: list val), *)
+(*       instant_same_clock xs -> *)
+(*       ~ absent_list xs -> *)
+(*       present_list xs. *)
+(*   Proof. *)
+(*     intros ** Hsamexs Hnabs. *)
+(*     now destruct Hsamexs. *)
+(*   Qed. *)
+
+(*   Lemma sem_vars_gt0: *)
+(*     forall H (xs: list (ident * type)) ls, *)
+(*       0 < length xs -> *)
+(*       sem_vars H (map fst xs) ls -> *)
+(*       forall n, 0 < length (ls n). *)
+(*   Proof. *)
+(*     intros ** Hgt0 Hsem n. *)
+(*     specialize (Hsem n). *)
+(*     apply Forall2_length in Hsem. *)
+(*     rewrite map_length in Hsem. *)
+(*     now rewrite Hsem in Hgt0. *)
+(*   Qed. *)
+
+(*   Ltac assert_const_length xss := *)
+(*     match goal with *)
+(*       H: sem_vars _ _ xss |- _ => *)
+(*       let H' := fresh in *)
+(*       let k := fresh in *)
+(*       let k' := fresh in *)
+(*       assert (wf_streams xss) *)
+(*         by (intros k k'; pose proof H as H'; *)
+(*             unfold sem_vars, lift in *; *)
+(*             specialize (H k); specialize (H' k'); *)
+(*             apply Forall2_length in H; apply Forall2_length in H'; *)
+(*             now rewrite H in H') *)
+(*     end. *)
+
+(*   (** ** Determinism of the semantics *) *)
+
+(*   (** *** Instantaneous semantics *) *)
+
+(*   Section InstantDeterminism. *)
+
+(*     Variable base: bool. *)
+(*     Variable R: env. *)
+(*     Variable S: state. *)
+
+(*     Lemma sem_var_var_instant_det: *)
+(*       forall x v1 v2, *)
+(*         sem_var_var_instant R x v1 *)
+(*         -> sem_var_var_instant R x v2 *)
+(*         -> v1 = v2. *)
 (*     Proof. *)
-(*       intros ** Hpoint H1 H2. *)
-(*       extensionality n. specialize (H1 n). specialize (H2 n). *)
-(*       eapply Hpoint; eassumption. *)
+(*       intros x v1 v2 H1 H2. *)
+(*       inversion_clear H1 as [Hf1]; *)
+(*         inversion_clear H2 as [Hf2]; *)
+(*         congruence. *)
+(*     Qed. *)
+(*     Hint Resolve sem_var_var_instant_det. *)
+
+(*     Lemma sem_clock_state_var_var_instant_det: *)
+(*       (forall ck v1, *)
+(*           sem_clock_instant base R S ck v1 -> *)
+(*           forall v2, *)
+(*             sem_clock_instant base R S ck v2 -> *)
+(*             v1 = v2) *)
+(*       /\ *)
+(*       (forall ck x v1, *)
+(*           sem_state_var_instant base R S ck x v1 -> *)
+(*           forall v2, *)
+(*             sem_state_var_instant base R S ck x v2 -> *)
+(*             v1 = v2) *)
+(*       /\ *)
+(*       (forall ck x v1, *)
+(*           sem_var_instant base R S ck x v1 -> *)
+(*           forall v2, *)
+(*             sem_var_instant base R S ck x v2 -> *)
+(*             v1 = v2). *)
+(*     Proof. *)
+(*       apply sem_clock_state_var_var_mut. *)
+(*       - intro; now inversion 1. *)
+(*       - intros ** VarDet ?? Sem. *)
+(*         inversion Sem as [ | | |??? b' ? SVar]; subst; auto. *)
+(*         apply VarDet in SVar; inv SVar. *)
+(*         destruct b'; simpl in *; congruence. *)
+(*       - intros ** Sem; inv Sem; auto. *)
+(*       - intros ** VarDet ?? Sem. *)
+(*         inversion Sem as [ |????? SVar| |]; subst; auto. *)
+(*         apply VarDet in SVar; inv SVar. *)
+(*         destruct b; simpl in *; congruence. *)
+(*       - intros ** ClockDet ? Sem. *)
+(*         inversion_clear Sem as [|??? SClock]; try congruence. *)
+(*         apply ClockDet in SClock; discriminate. *)
+(*       - intros ** ClockDet ? Sem. *)
+(*         inversion_clear Sem as [???? SClock|]; auto. *)
+(*         apply ClockDet in SClock; discriminate. *)
+(*       - intros ** Sem; inv Sem; eauto. *)
+(*       - intros ** Sem; inv Sem; auto. *)
 (*     Qed. *)
 
-(*     Ltac apply_lift sem_det := *)
-(*       intros; eapply lift_det; try eassumption; *)
-(*       compute; intros; eapply sem_det; eauto. *)
-
-(*     Ltac apply_lift' sem_det := *)
-(*       intros; eapply lift'_det; try eassumption; *)
-(*       compute; intros; eapply sem_det; eauto. *)
-
-(*     Lemma sem_var_det: *)
-(*       forall x xs1 xs2, *)
-(*         sem_var H x xs1 -> sem_var H x xs2 -> xs1 = xs2. *)
+(*     Corollary sem_clock_instant_det: *)
+(*       forall ck v1 v2, *)
+(*         sem_clock_instant base R S ck v1 *)
+(*         -> sem_clock_instant base R S ck v2 *)
+(*         -> v1 = v2. *)
 (*     Proof. *)
-(*       apply_lift' sem_var_instant_det. *)
+(*       intros; eapply sem_clock_state_var_var_instant_det; eauto. *)
+(*     Qed. *)
+(*     Hint Resolve sem_clock_instant_det. *)
+
+(*     Corollary sem_state_var_instant_det: *)
+(*       forall x ck v1 v2, *)
+(*         sem_state_var_instant base R S ck x v1 *)
+(*         -> sem_state_var_instant base R S ck x v2 *)
+(*         -> v1 = v2. *)
+(*     Proof. *)
+(*       intros; eapply (proj1 (proj2 sem_clock_state_var_var_instant_det)); eauto. *)
+(*     Qed. *)
+(*     Hint Resolve sem_state_var_instant_det. *)
+
+(*     Corollary sem_var_instant_det: *)
+(*       forall x ck v1 v2, *)
+(*         sem_var_instant base R S ck x v1 *)
+(*         -> sem_var_instant base R S ck x v2 *)
+(*         -> v1 = v2. *)
+(*     Proof. *)
+(*       intros; eapply sem_clock_state_var_var_instant_det; eauto. *)
+(*     Qed. *)
+(*     Hint Resolve sem_var_instant_det. *)
+
+(*     Lemma sem_lexp_instant_det: *)
+(*       forall e ck v1 v2, *)
+(*         sem_lexp_instant base R S ck e v1 *)
+(*         -> sem_lexp_instant base R S ck e v2 *)
+(*         -> v1 = v2. *)
+(*     Proof. *)
+(*       induction e (* using lexp_ind2 *). *)
+(*       - (* Econst *) *)
+(*         do 2 inversion_clear 1; destruct base; congruence. *)
+(*       - (* Evar *) *)
+(*         intros ** S1 S2; inv S1; inv S2; eauto. *)
+(*       - (* Ewhen *) *)
+(*         intros ** S1 S2; inv S1; inv S2; eauto; *)
+(*           repeat progress match goal with *)
+(*                           | H1:sem_lexp_instant ?b ?R ?S ?ck ?e ?v1, *)
+(*                                H2:sem_lexp_instant ?b ?R ?S ?ck ?e ?v2 |- _ => *)
+(*                             apply IHe with (1:=H1) in H2 *)
+(*                           | H1:sem_var_instant ?b ?R ?S ?ck ?i ?v1, *)
+(*                                H2:sem_var_instant ?b ?R ?S ?ck ?i ?v2 |- _ => *)
+(*                             apply sem_var_instant_det with (1:=H1) in H2 *)
+(*                           | Hp:present _ = present _ |- _ => *)
+(*                             injection Hp; intro; subst *)
+(*                           | H1:val_to_bool _ = Some _, *)
+(*                                H2:val_to_bool _ = Some (negb _) |- _ => *)
+(*                             rewrite H2 in H1; exfalso; injection H1; *)
+(*                               now apply Bool.no_fixpoint_negb *)
+(*                           end; subst; auto. *)
+(*       - (* Eunop *) *)
+(*         intros ** S1 S2; inv S1; inv S2; *)
+(*           repeat progress match goal with *)
+(*                           | H1:sem_lexp_instant _ _ _ _ e _, H2:sem_lexp_instant _ _ _ _ e _ |- _ => *)
+(*                             apply IHe with (1:=H1) in H2; inversion H2; subst *)
+(*                           | H1:sem_unop _ _ _ = _, H2:sem_unop _ _ _ = _ |- _ => *)
+(*                             rewrite H1 in H2; injection H2; intro; subst *)
+(*                           | H1:sem_lexp_instant _ _ _ _ _ (present _), *)
+(*                                H2:sem_lexp_instant _ _ _ _ _ absent |- _ => *)
+(*                             apply IHe with (1:=H1) in H2 *)
+(*                           end; try auto. *)
+(*       - (* Ebinop *) *)
+(*         intros ** S1 S2; inv S1; inv S2; *)
+(*           repeat progress match goal with *)
+(*                           | H1:sem_lexp_instant _ _ _ _ e1 _, H2:sem_lexp_instant _ _ _ _ e1 _ |- _ => *)
+(*                             apply IHe1 with (1:=H1) in H2 *)
+(*                           | H1:sem_lexp_instant _ _ _ _ e2 _, H2:sem_lexp_instant _ _ _ _ e2 _ |- _ => *)
+(*                             apply IHe2 with (1:=H1) in H2 *)
+(*                           | H1:sem_binop _ _ _ _ _ = Some ?v1, *)
+(*                                H2:sem_binop _ _ _ _ _ = Some ?v2 |- _ => *)
+(*                             rewrite H1 in H2; injection H2; intro; subst *)
+(*                           | H:present _ = present _ |- _ => injection H; intro; subst *)
+(*                           end; subst; auto; discriminate. *)
+(*     Qed. *)
+(*     Hint Resolve sem_lexp_instant_det. *)
+
+(*     Lemma sem_laexp_instant_det: *)
+(*       forall ck e v1 v2, *)
+(*         sem_laexp_instant base R S ck e v1 *)
+(*         -> sem_laexp_instant base R S ck e v2 *)
+(*         -> v1 = v2. *)
+(*     Proof. *)
+(*       do 2 inversion_clear 1; eauto. *)
 (*     Qed. *)
 
-(*     Lemma sem_clock_det: *)
-(*       forall ck bs1 bs2, *)
-(*         sem_clock bk H ck bs1 -> sem_clock bk H ck bs2 -> bs1 = bs2. *)
-(*     Proof. *)
-(*       apply_lift sem_clock_instant_det. *)
-(*     Qed. *)
-
-(*     Lemma sem_lexp_det: *)
-(*       forall e xs1 xs2, *)
-(*         sem_lexp bk H e xs1 -> sem_lexp bk H e xs2 -> xs1 = xs2. *)
-(*     Proof. *)
-(*       apply_lift sem_lexp_instant_det. *)
-(*     Qed. *)
-
-(*     Lemma sem_lexps_det: *)
-(*       forall les cs1 cs2, *)
-(*         sem_lexps bk H les cs1 -> *)
-(*         sem_lexps bk H les cs2 -> *)
+(*     Lemma sem_lexps_instant_det: *)
+(*       forall les ck cs1 cs2, *)
+(*         sem_lexps_instant base R S ck les cs1 -> *)
+(*         sem_lexps_instant base R S ck les cs2 -> *)
 (*         cs1 = cs2. *)
 (*     Proof. *)
-(*       apply_lift sem_lexps_instant_det. *)
+(*       intros ???; eapply Forall2_det; eauto. *)
 (*     Qed. *)
+(*     Hint Resolve sem_lexps_instant_det. *)
 
-(*     Lemma sem_laexp_det: *)
-(*       forall ck e xs1 xs2, *)
-(*         sem_laexp bk H ck e xs1 -> sem_laexp bk H ck e xs2 -> xs1 = xs2. *)
+(*     Lemma sem_laexps_instant_det: *)
+(*       forall ck e v1 v2, *)
+(*         sem_laexps_instant base R S ck e v1 *)
+(*         -> sem_laexps_instant base R S ck e v2 *)
+(*         -> v1 = v2. *)
 (*     Proof. *)
-(*       apply_lift sem_laexp_instant_det. *)
+(*       do 2 inversion_clear 1; eauto. *)
 (*     Qed. *)
 
-(*     Lemma sem_laexps_det: *)
-(*       forall ck e xs1 xs2, *)
-(*         sem_laexps bk H ck e xs1 -> sem_laexps bk H ck e xs2 -> xs1 = xs2. *)
+(*     Lemma sem_cexp_instant_det: *)
+(*       forall e ck v1 v2, *)
+(*         sem_cexp_instant base R S ck e v1 *)
+(*         -> sem_cexp_instant base R S ck e v2 *)
+(*         -> v1 = v2. *)
 (*     Proof. *)
-(*       apply_lift sem_laexps_instant_det. *)
+(*       induction e; *)
+(*         do 2 inversion_clear 1; *)
+(*         try repeat progress match goal with *)
+(*                             | H1: sem_cexp_instant ?bk ?R ?S ?ck ?e ?l, *)
+(*                                   H2: sem_cexp_instant ?bk ?R ?S ?ck ?e ?r |- _ => *)
+(*                               apply IHe1 with (1:=H1) in H2 *)
+(*                                                          || apply IHe2 with (1:=H1) in H2; *)
+(*                                 injection H2; intro; subst *)
+(*                             | H1: sem_var_instant ?b ?R ?S ?ck ?i (present true_val), *)
+(*                                   H2: sem_var_instant ?b ?R ?S ?ck ?i (present false_val) |- _ => *)
+(*                               apply sem_var_instant_det with (1:=H1) in H2; *)
+(*                                 exfalso; injection H2; now apply true_not_false_val *)
+(*                             | H1: sem_lexp_instant ?bk ?R ?S ?ck ?l ?v1, *)
+(*                                   H2: sem_lexp_instant ?bk ?R ?S ?ck ?l ?v2 |- _ => *)
+(*                               apply sem_lexp_instant_det with (1:=H1) in H2; *)
+(*                                 discriminate || injection H2; intro; subst *)
+(*                             | H1: sem_var_instant ?bk ?R ?S ?ck ?i (present _), *)
+(*                                   H2: sem_var_instant ?bk ?R ?S ?ck ?i absent |- _ => *)
+(*                               apply sem_var_instant_det with (1:=H1) in H2; discriminate *)
+(*                             | H1: val_to_bool _ = Some _, *)
+(*                                   H2:val_to_bool _ = Some _ |- _ => *)
+(*                               rewrite H1 in H2; injection H2; intro; subst *)
+(*                             end; eauto. *)
 (*     Qed. *)
+(*     Hint Resolve sem_cexp_instant_det. *)
 
-(*     Lemma sem_cexp_det: *)
-(*       forall c xs1 xs2, *)
-(*         sem_cexp bk H c xs1 -> sem_cexp bk H c xs2 -> xs1 = xs2. *)
+(*     Lemma sem_caexp_instant_det: *)
+(*       forall ck e v1 v2, *)
+(*         sem_caexp_instant base R S ck e v1 *)
+(*         -> sem_caexp_instant base R S ck e v2 *)
+(*         -> v1 = v2. *)
 (*     Proof. *)
-(*       apply_lift sem_cexp_instant_det. *)
+(*       intros until v2. *)
+(*       do 2 inversion_clear 1; eauto. *)
 (*     Qed. *)
 
-(*     Lemma sem_caexp_det: *)
-(*       forall ck c xs1 xs2, *)
-(*         sem_caexp bk H ck c xs1 -> sem_caexp bk H ck c xs2 -> xs1 = xs2. *)
-(*     Proof. *)
-(*       apply_lift sem_caexp_instant_det. *)
-(*     Qed. *)
+(*   End InstantDeterminism. *)
 
-(*   (* XXX: every semantics definition, including [sem_var] which doesn't *)
-(* need it, takes a base clock value or base clock stream, except *)
-(* [sem_var_instant]. For uniformity, we may want to pass a (useless) *)
-(* clock to [sem_var_instant] too. *) *)
+(*   (** *** Lifted semantics *) *)
 
-(*   End LiftDeterminism. *)
+(*   (* Section LiftDeterminism. *) *)
 
-  (* Ltac sem_det := *)
-  (*   match goal with *)
-  (*   | H1: sem_clock_instant ?bk ?H ?C ?X, *)
-  (*         H2: sem_clock_instant ?bk ?H ?C ?Y |- ?X = ?Y => *)
-  (*     eapply sem_clock_instant_det; eexact H1 || eexact H2 *)
-  (*   | H1: sem_clock ?bk ?H ?C ?X, *)
-  (*         H2: sem_clock ?bk ?H ?C ?Y |- ?X = ?Y => *)
-  (*     eapply sem_clock_det; eexact H1 || eexact H2 *)
-  (*   | H1: sem_cexp_instant ?bk ?H ?C ?X, *)
-  (*         H2: sem_cexp_instant ?bk ?H ?C ?Y |- ?X = ?Y => *)
-  (*     eapply sem_cexp_instant_det; eexact H1 || eexact H2 *)
-  (*   | H1: sem_cexp ?bk ?H ?C ?X, *)
-  (*         H2: sem_cexp ?bk ?H ?C ?Y |- ?X = ?Y => *)
-  (*     eapply sem_cexp_det; eexact H1 || eexact H2 *)
-  (*   | H1: sem_lexps_instant ?bk ?H ?C ?X, *)
-  (*         H2: sem_lexps_instant ?bk ?H ?C ?Y |- ?X = ?Y => *)
-  (*     eapply sem_lexps_instant_det; eexact H1 || eexact H2 *)
-  (*   | H1: sem_lexps ?bk ?H ?C ?X, *)
-  (*         H2: sem_lexps ?bk ?H ?C ?Y |- ?X = ?Y => *)
-  (*     eapply sem_lexps_det; eexact H1 || eexact H2 *)
-  (*   | H1: sem_laexps_instant ?bk ?H ?ck ?C ?X, *)
-  (*         H2: sem_laexps_instant ?bk ?H ?ck ?C ?Y |- ?X = ?Y => *)
-  (*     eapply sem_laexps_instant_det; eexact H1 || eexact H2 *)
-  (*   | H1: sem_laexps ?bk ?H ?ck ?C ?X, *)
-  (*         H2: sem_laexps ?bk ?H ?ck ?C ?Y |- ?X = ?Y => *)
-  (*     eapply sem_laexps_det; eexact H1 || eexact H2 *)
-  (*   | H1: sem_lexp_instant ?bk ?H ?C ?X, *)
-  (*         H2: sem_lexp_instant ?bk ?H ?C ?Y |- ?X = ?Y => *)
-  (*     eapply sem_lexp_instant_det; eexact H1 || eexact H2 *)
-  (*   | H1: sem_lexp ?bk ?H ?C ?X, *)
-  (*         H2: sem_lexp ?bk ?H ?C ?Y |- ?X = ?Y => *)
-  (*     eapply sem_lexp_det; eexact H1 || eexact H2 *)
-  (*   | H1: sem_laexp_instant ?bk ?H ?CK ?C ?X, *)
-  (*         H2: sem_laexp_instant ?bk ?H ?CK ?C ?Y |- ?X = ?Y => *)
-  (*     eapply sem_laexp_instant_det; eexact H1 || eexact H2 *)
-  (*   | H1: sem_laexp ?bk ?H ?CK ?C ?X, *)
-  (*         H2: sem_laexp ?bk ?H ?CK ?C ?Y |- ?X = ?Y => *)
-  (*     eapply sem_laexp_det; eexact H1 || eexact H2 *)
-  (*   | H1: sem_var_instant ?H ?C ?X, *)
-  (*         H2: sem_var_instant ?H ?C ?Y |- ?X = ?Y => *)
-  (*     eapply sem_var_instant_det; eexact H1 || eexact H2 *)
-  (*   | H1: sem_var ?H ?C ?X, *)
-  (*         H2: sem_var ?H ?C ?Y |- ?X = ?Y => *)
-  (*     eapply sem_var_det; eexact H1 || eexact H2 *)
-  (*   end. *)
-  (* Record mvalue := *)
-  (*   Mvalue { content_i: val; *)
-  (*            reset_i: bool *)
-  (*          }. *)
+(* (*     Variable bk : stream bool. *) *)
+(* (*     Variable H : history. *) *)
+
+(* (*     Require Import Logic.FunctionalExtensionality. *) *)
+
+(* (*     Lemma lift_det: *) *)
+(* (*       forall {A B} (P: bool -> env -> A -> B -> Prop) (bk: stream bool) *) *)
+(* (*         x (xs1 xs2 : stream B), *) *)
+(* (*         (forall b R v1 v2, P b R x v1 -> P b R x v2 -> v1 = v2) -> *) *)
+(* (*         lift bk H P x xs1 -> lift bk H P x xs2 -> xs1 = xs2. *) *)
+(* (*     Proof. *) *)
+(* (*       intros ** Hpoint H1 H2. *) *)
+(* (*       extensionality n. specialize (H1 n). specialize (H2 n). *) *)
+(* (*       eapply Hpoint; eassumption. *) *)
+(* (*     Qed. *) *)
+
+(* (*     Lemma lift'_det: *) *)
+(* (*       forall {A B} (P: env -> A -> B -> Prop) *) *)
+(* (*         x (xs1 xs2 : stream B), *) *)
+(* (*         (forall R v1 v2, P R x v1 -> P R x v2 -> v1 = v2) -> *) *)
+(* (*         lift' H P x xs1 -> lift' H P x xs2 -> xs1 = xs2. *) *)
+(* (*     Proof. *) *)
+(* (*       intros ** Hpoint H1 H2. *) *)
+(* (*       extensionality n. specialize (H1 n). specialize (H2 n). *) *)
+(* (*       eapply Hpoint; eassumption. *) *)
+(* (*     Qed. *) *)
+
+(* (*     Ltac apply_lift sem_det := *) *)
+(* (*       intros; eapply lift_det; try eassumption; *) *)
+(* (*       compute; intros; eapply sem_det; eauto. *) *)
+
+(* (*     Ltac apply_lift' sem_det := *) *)
+(* (*       intros; eapply lift'_det; try eassumption; *) *)
+(* (*       compute; intros; eapply sem_det; eauto. *) *)
+
+(* (*     Lemma sem_var_det: *) *)
+(* (*       forall x xs1 xs2, *) *)
+(* (*         sem_var H x xs1 -> sem_var H x xs2 -> xs1 = xs2. *) *)
+(* (*     Proof. *) *)
+(* (*       apply_lift' sem_var_instant_det. *) *)
+(* (*     Qed. *) *)
+
+(* (*     Lemma sem_clock_det: *) *)
+(* (*       forall ck bs1 bs2, *) *)
+(* (*         sem_clock bk H ck bs1 -> sem_clock bk H ck bs2 -> bs1 = bs2. *) *)
+(* (*     Proof. *) *)
+(* (*       apply_lift sem_clock_instant_det. *) *)
+(* (*     Qed. *) *)
+
+(* (*     Lemma sem_lexp_det: *) *)
+(* (*       forall e xs1 xs2, *) *)
+(* (*         sem_lexp bk H e xs1 -> sem_lexp bk H e xs2 -> xs1 = xs2. *) *)
+(* (*     Proof. *) *)
+(* (*       apply_lift sem_lexp_instant_det. *) *)
+(* (*     Qed. *) *)
+
+(* (*     Lemma sem_lexps_det: *) *)
+(* (*       forall les cs1 cs2, *) *)
+(* (*         sem_lexps bk H les cs1 -> *) *)
+(* (*         sem_lexps bk H les cs2 -> *) *)
+(* (*         cs1 = cs2. *) *)
+(* (*     Proof. *) *)
+(* (*       apply_lift sem_lexps_instant_det. *) *)
+(* (*     Qed. *) *)
+
+(* (*     Lemma sem_laexp_det: *) *)
+(* (*       forall ck e xs1 xs2, *) *)
+(* (*         sem_laexp bk H ck e xs1 -> sem_laexp bk H ck e xs2 -> xs1 = xs2. *) *)
+(* (*     Proof. *) *)
+(* (*       apply_lift sem_laexp_instant_det. *) *)
+(* (*     Qed. *) *)
+
+(* (*     Lemma sem_laexps_det: *) *)
+(* (*       forall ck e xs1 xs2, *) *)
+(* (*         sem_laexps bk H ck e xs1 -> sem_laexps bk H ck e xs2 -> xs1 = xs2. *) *)
+(* (*     Proof. *) *)
+(* (*       apply_lift sem_laexps_instant_det. *) *)
+(* (*     Qed. *) *)
+
+(* (*     Lemma sem_cexp_det: *) *)
+(* (*       forall c xs1 xs2, *) *)
+(* (*         sem_cexp bk H c xs1 -> sem_cexp bk H c xs2 -> xs1 = xs2. *) *)
+(* (*     Proof. *) *)
+(* (*       apply_lift sem_cexp_instant_det. *) *)
+(* (*     Qed. *) *)
+
+(* (*     Lemma sem_caexp_det: *) *)
+(* (*       forall ck c xs1 xs2, *) *)
+(* (*         sem_caexp bk H ck c xs1 -> sem_caexp bk H ck c xs2 -> xs1 = xs2. *) *)
+(* (*     Proof. *) *)
+(* (*       apply_lift sem_caexp_instant_det. *) *)
+(* (*     Qed. *) *)
+
+(* (*   (* XXX: every semantics definition, including [sem_var] which doesn't *) *)
+(* (* need it, takes a base clock value or base clock stream, except *) *)
+(* (* [sem_var_instant]. For uniformity, we may want to pass a (useless) *) *)
+(* (* clock to [sem_var_instant] too. *) *) *)
+
+(* (*   End LiftDeterminism. *) *)
+
+(*   (* Ltac sem_det := *) *)
+(*   (*   match goal with *) *)
+(*   (*   | H1: sem_clock_instant ?bk ?H ?C ?X, *) *)
+(*   (*         H2: sem_clock_instant ?bk ?H ?C ?Y |- ?X = ?Y => *) *)
+(*   (*     eapply sem_clock_instant_det; eexact H1 || eexact H2 *) *)
+(*   (*   | H1: sem_clock ?bk ?H ?C ?X, *) *)
+(*   (*         H2: sem_clock ?bk ?H ?C ?Y |- ?X = ?Y => *) *)
+(*   (*     eapply sem_clock_det; eexact H1 || eexact H2 *) *)
+(*   (*   | H1: sem_cexp_instant ?bk ?H ?C ?X, *) *)
+(*   (*         H2: sem_cexp_instant ?bk ?H ?C ?Y |- ?X = ?Y => *) *)
+(*   (*     eapply sem_cexp_instant_det; eexact H1 || eexact H2 *) *)
+(*   (*   | H1: sem_cexp ?bk ?H ?C ?X, *) *)
+(*   (*         H2: sem_cexp ?bk ?H ?C ?Y |- ?X = ?Y => *) *)
+(*   (*     eapply sem_cexp_det; eexact H1 || eexact H2 *) *)
+(*   (*   | H1: sem_lexps_instant ?bk ?H ?C ?X, *) *)
+(*   (*         H2: sem_lexps_instant ?bk ?H ?C ?Y |- ?X = ?Y => *) *)
+(*   (*     eapply sem_lexps_instant_det; eexact H1 || eexact H2 *) *)
+(*   (*   | H1: sem_lexps ?bk ?H ?C ?X, *) *)
+(*   (*         H2: sem_lexps ?bk ?H ?C ?Y |- ?X = ?Y => *) *)
+(*   (*     eapply sem_lexps_det; eexact H1 || eexact H2 *) *)
+(*   (*   | H1: sem_laexps_instant ?bk ?H ?ck ?C ?X, *) *)
+(*   (*         H2: sem_laexps_instant ?bk ?H ?ck ?C ?Y |- ?X = ?Y => *) *)
+(*   (*     eapply sem_laexps_instant_det; eexact H1 || eexact H2 *) *)
+(*   (*   | H1: sem_laexps ?bk ?H ?ck ?C ?X, *) *)
+(*   (*         H2: sem_laexps ?bk ?H ?ck ?C ?Y |- ?X = ?Y => *) *)
+(*   (*     eapply sem_laexps_det; eexact H1 || eexact H2 *) *)
+(*   (*   | H1: sem_lexp_instant ?bk ?H ?C ?X, *) *)
+(*   (*         H2: sem_lexp_instant ?bk ?H ?C ?Y |- ?X = ?Y => *) *)
+(*   (*     eapply sem_lexp_instant_det; eexact H1 || eexact H2 *) *)
+(*   (*   | H1: sem_lexp ?bk ?H ?C ?X, *) *)
+(*   (*         H2: sem_lexp ?bk ?H ?C ?Y |- ?X = ?Y => *) *)
+(*   (*     eapply sem_lexp_det; eexact H1 || eexact H2 *) *)
+(*   (*   | H1: sem_laexp_instant ?bk ?H ?CK ?C ?X, *) *)
+(*   (*         H2: sem_laexp_instant ?bk ?H ?CK ?C ?Y |- ?X = ?Y => *) *)
+(*   (*     eapply sem_laexp_instant_det; eexact H1 || eexact H2 *) *)
+(*   (*   | H1: sem_laexp ?bk ?H ?CK ?C ?X, *) *)
+(*   (*         H2: sem_laexp ?bk ?H ?CK ?C ?Y |- ?X = ?Y => *) *)
+(*   (*     eapply sem_laexp_det; eexact H1 || eexact H2 *) *)
+(*   (*   | H1: sem_var_instant ?H ?C ?X, *) *)
+(*   (*         H2: sem_var_instant ?H ?C ?Y |- ?X = ?Y => *) *)
+(*   (*     eapply sem_var_instant_det; eexact H1 || eexact H2 *) *)
+(*   (*   | H1: sem_var ?H ?C ?X, *) *)
+(*   (*         H2: sem_var ?H ?C ?Y |- ?X = ?Y => *) *)
+(*   (*     eapply sem_var_det; eexact H1 || eexact H2 *) *)
+(*   (*   end. *) *)
+(*   (* Record mvalue := *) *)
+(*   (*   Mvalue { content_i: val; *) *)
+(*   (*            reset_i: bool *) *)
+(*   (*          }. *) *)
 
 
-  (** Morphisms properties *)
+(*   (** Morphisms properties *) *)
 
-  Add Parametric Morphism P b E E': (fun xss yss => sem_block P b E xss yss E')
-      with signature eq_str ==> eq_str ==> Basics.impl
-        as sem_node_eq_str.
-  Proof.
-    intros ** E1 ? ? E2 Block.
-    inv Block.
-    econstructor; eauto; intro; try rewrite <-E1; try rewrite <-E2; auto.
-  Qed.
+(*   Add Parametric Morphism P b E E': (fun xss yss => sem_block P b E xss yss E') *)
+(*       with signature eq_str ==> eq_str ==> Basics.impl *)
+(*         as sem_node_eq_str. *)
+(*   Proof. *)
+(*     intros ** E1 ? ? E2 Block. *)
+(*     inv Block. *)
+(*     econstructor; eauto; intro; try rewrite <-E1; try rewrite <-E2; auto. *)
+(*   Qed. *)
 
-  Lemma sem_block_wf:
-    forall P f E E' xss yss,
-      sem_block P f E xss yss E' ->
-      wf_streams xss /\ wf_streams yss.
-  Proof.
-    intros ** Sem; split; inv Sem;
-      assert_const_length xss; assert_const_length yss; auto.
-  Qed.
+(*   Lemma sem_block_wf: *)
+(*     forall P f E E' xss yss, *)
+(*       sem_block P f E xss yss E' -> *)
+(*       wf_streams xss /\ wf_streams yss. *)
+(*   Proof. *)
+(*     intros ** Sem; split; inv Sem; *)
+(*       assert_const_length xss; assert_const_length yss; auto. *)
+(*   Qed. *)
 
-  (* Lemma sem_EqCall_gt0: *)
-  (*   forall P bk H M xs ck b i es, *)
-  (*     sem_equation P bk H M (EqCall xs ck b i es) -> *)
-  (*     0 < length xs. *)
-  (* Proof. *)
-  (*   inversion_clear 1 as [| | |????????????? Block' Vars]. *)
-  (*   inversion_clear Block' as [??????????? Out]. *)
-  (*   specialize (Out 0); specialize (Vars 0); simpl in *; *)
-  (*     apply Forall2_length in Out; apply Forall2_length in Vars. *)
-  (*   rewrite <-Out in Vars; rewrite Vars, map_length; apply b_outgt0. *)
-  (* Qed. *)
+(*   (* Lemma sem_EqCall_gt0: *) *)
+(*   (*   forall P bk H M xs ck b i es, *) *)
+(*   (*     sem_equation P bk H M (EqCall xs ck b i es) -> *) *)
+(*   (*     0 < length xs. *) *)
+(*   (* Proof. *) *)
+(*   (*   inversion_clear 1 as [| | |????????????? Block' Vars]. *) *)
+(*   (*   inversion_clear Block' as [??????????? Out]. *) *)
+(*   (*   specialize (Out 0); specialize (Vars 0); simpl in *; *) *)
+(*   (*     apply Forall2_length in Out; apply Forall2_length in Vars. *) *)
+(*   (*   rewrite <-Out in Vars; rewrite Vars, map_length; apply b_outgt0. *) *)
+(*   (* Qed. *) *)
 
-  (* Lemma In_fold_left_fby_eq: *)
-  (*   forall x eqs m, *)
-  (*     PS.In x (fold_left fby_eq eqs m) *)
-  (*     <-> PS.In x (fbys eqs) \/ PS.In x m. *)
-  (* Proof. *)
-  (*   unfold fbys. *)
-  (*   induction eqs as [|eq]. *)
-  (*   - split; auto. *)
-  (*     destruct 1 as [H|]. *)
-  (*     apply not_In_empty in H; contradiction. *)
-  (*     auto. *)
-  (*   - split. *)
-  (*     + intro H. *)
-  (*       simpl; rewrite IHeqs. *)
-  (*       simpl in H; apply IHeqs in H; destruct H; auto. *)
-  (*       destruct eq; auto. *)
-  (*       apply PS.add_spec in H. *)
-  (*       destruct H. *)
-  (*       rewrite H; left; right; apply PS.add_spec; intuition. *)
-  (*       intuition. *)
-  (*     + destruct 1 as [H|H]. *)
-  (*       * simpl in H; rewrite IHeqs in H; apply IHeqs; destruct H; auto. *)
-  (*         right. *)
-  (*         destruct eq; try (apply not_In_empty in H; contradiction). *)
-  (*         simpl; apply PS.add_spec. *)
-  (*         apply PS.add_spec in H; destruct H; *)
-  (*           try apply not_In_empty in H; intuition. *)
-  (*       * apply IHeqs; right; destruct eq; auto. *)
-  (*         apply PS.add_spec; auto. *)
-  (* Qed. *)
+(*   (* Lemma In_fold_left_fby_eq: *) *)
+(*   (*   forall x eqs m, *) *)
+(*   (*     PS.In x (fold_left fby_eq eqs m) *) *)
+(*   (*     <-> PS.In x (fbys eqs) \/ PS.In x m. *) *)
+(*   (* Proof. *) *)
+(*   (*   unfold fbys. *) *)
+(*   (*   induction eqs as [|eq]. *) *)
+(*   (*   - split; auto. *) *)
+(*   (*     destruct 1 as [H|]. *) *)
+(*   (*     apply not_In_empty in H; contradiction. *) *)
+(*   (*     auto. *) *)
+(*   (*   - split. *) *)
+(*   (*     + intro H. *) *)
+(*   (*       simpl; rewrite IHeqs. *) *)
+(*   (*       simpl in H; apply IHeqs in H; destruct H; auto. *) *)
+(*   (*       destruct eq; auto. *) *)
+(*   (*       apply PS.add_spec in H. *) *)
+(*   (*       destruct H. *) *)
+(*   (*       rewrite H; left; right; apply PS.add_spec; intuition. *) *)
+(*   (*       intuition. *) *)
+(*   (*     + destruct 1 as [H|H]. *) *)
+(*   (*       * simpl in H; rewrite IHeqs in H; apply IHeqs; destruct H; auto. *) *)
+(*   (*         right. *) *)
+(*   (*         destruct eq; try (apply not_In_empty in H; contradiction). *) *)
+(*   (*         simpl; apply PS.add_spec. *) *)
+(*   (*         apply PS.add_spec in H; destruct H; *) *)
+(*   (*           try apply not_In_empty in H; intuition. *) *)
+(*   (*       * apply IHeqs; right; destruct eq; auto. *) *)
+(*   (*         apply PS.add_spec; auto. *) *)
+(*   (* Qed. *) *)
 
-  (* Lemma In_fold_left_inst_eq: *)
-  (*   forall x eqs m, *)
-  (*     PS.In x (fold_left inst_eq eqs m) *)
-  (*     <-> PS.In x (insts eqs) \/ PS.In x m. *)
-  (* Proof. *)
-  (*   unfold insts. *)
-  (*   induction eqs as [|eq]. *)
-  (*   - split; auto. *)
-  (*     destruct 1 as [H|]. *)
-  (*     apply not_In_empty in H; contradiction. *)
-  (*     auto. *)
-  (*   - split. *)
-  (*     + intro H. *)
-  (*       simpl; rewrite IHeqs. *)
-  (*       simpl in H; apply IHeqs in H; destruct H; auto. *)
-  (*       destruct eq; auto; apply PS.add_spec in H; destruct H; auto; *)
-  (*         rewrite H; left; right; apply PS.add_spec; auto. *)
-  (*     + destruct 1 as [H|H]. *)
-  (*       * simpl in H; rewrite IHeqs in H; apply IHeqs; destruct H; auto. *)
-  (*         right. *)
-  (*         destruct eq; try (apply not_In_empty in H; contradiction); *)
-  (*           simpl; apply PS.add_spec; *)
-  (*             apply PS.add_spec in H; destruct H; auto; *)
-  (*               apply not_In_empty in H; contradiction. *)
-  (*       * apply IHeqs; right; destruct eq; auto; *)
-  (*           apply PS.add_spec; auto. *)
-  (* Qed. *)
+(*   (* Lemma In_fold_left_inst_eq: *) *)
+(*   (*   forall x eqs m, *) *)
+(*   (*     PS.In x (fold_left inst_eq eqs m) *) *)
+(*   (*     <-> PS.In x (insts eqs) \/ PS.In x m. *) *)
+(*   (* Proof. *) *)
+(*   (*   unfold insts. *) *)
+(*   (*   induction eqs as [|eq]. *) *)
+(*   (*   - split; auto. *) *)
+(*   (*     destruct 1 as [H|]. *) *)
+(*   (*     apply not_In_empty in H; contradiction. *) *)
+(*   (*     auto. *) *)
+(*   (*   - split. *) *)
+(*   (*     + intro H. *) *)
+(*   (*       simpl; rewrite IHeqs. *) *)
+(*   (*       simpl in H; apply IHeqs in H; destruct H; auto. *) *)
+(*   (*       destruct eq; auto; apply PS.add_spec in H; destruct H; auto; *) *)
+(*   (*         rewrite H; left; right; apply PS.add_spec; auto. *) *)
+(*   (*     + destruct 1 as [H|H]. *) *)
+(*   (*       * simpl in H; rewrite IHeqs in H; apply IHeqs; destruct H; auto. *) *)
+(*   (*         right. *) *)
+(*   (*         destruct eq; try (apply not_In_empty in H; contradiction); *) *)
+(*   (*           simpl; apply PS.add_spec; *) *)
+(*   (*             apply PS.add_spec in H; destruct H; auto; *) *)
+(*   (*               apply not_In_empty in H; contradiction. *) *)
+(*   (*       * apply IHeqs; right; destruct eq; auto; *) *)
+(*   (*           apply PS.add_spec; auto. *) *)
+(*   (* Qed. *) *)
 
-  (* Lemma well_structured_def: *)
-  (*   forall M x ck e eqs, *)
-  (*     well_structured_memories (EqDef x ck e :: eqs) M <-> *)
-  (*     well_structured_memories eqs M. *)
-  (* Proof. *)
-  (*   split; eauto. *)
-  (* Qed. *)
+(*   (* Lemma well_structured_def: *) *)
+(*   (*   forall M x ck e eqs, *) *)
+(*   (*     well_structured_memories (EqDef x ck e :: eqs) M <-> *) *)
+(*   (*     well_structured_memories eqs M. *) *)
+(*   (* Proof. *) *)
+(*   (*   split; eauto. *) *)
+(*   (* Qed. *) *)
 
-  (* Lemma well_structured_add_inst_call: *)
-  (*   forall M M' xs ck f i es eqs, *)
-  (*     well_structured_memories eqs M -> *)
-  (*     well_structured_memories (EqCall xs ck f i es :: eqs) (add_inst i M' M). *)
-  (* Proof. *)
-  (*   intros ** WS. *)
-  (*   constructor; unfold fbys, insts; simpl; split; intro H. *)
-  (*   - rewrite find_val_add_inst in H; apply WS in H; auto. *)
-  (*   - rewrite find_val_add_inst; apply WS in H; auto. *)
-  (*   - rewrite In_fold_left_inst_eq. *)
-  (*     destruct (ident_eqb x i) eqn: E; *)
-  (*       [apply ident_eqb_eq in E; subst|apply ident_eqb_neq in E]. *)
-  (*     + right; apply PSE.MP.Dec.F.add_1; auto. *)
-  (*     + rewrite find_inst_gso in H; auto. *)
-  (*       apply WS in H; auto. *)
-  (*   - destruct (ident_eqb x i) eqn: E; *)
-  (*       [apply ident_eqb_eq in E; subst|apply ident_eqb_neq in E]. *)
-  (*     + rewrite find_inst_gss; intro; discriminate. *)
-  (*     + rewrite find_inst_gso; auto. *)
-  (*       apply WS. *)
-  (*       apply In_fold_left_inst_eq in H as [|H]; auto. *)
-  (*       apply PSE.MP.Dec.F.add_3 in H; auto. *)
-  (*       contradict H; apply not_In_empty. *)
-  (* Qed. *)
+(*   (* Lemma well_structured_add_inst_call: *) *)
+(*   (*   forall M M' xs ck f i es eqs, *) *)
+(*   (*     well_structured_memories eqs M -> *) *)
+(*   (*     well_structured_memories (EqCall xs ck f i es :: eqs) (add_inst i M' M). *) *)
+(*   (* Proof. *) *)
+(*   (*   intros ** WS. *) *)
+(*   (*   constructor; unfold fbys, insts; simpl; split; intro H. *) *)
+(*   (*   - rewrite find_val_add_inst in H; apply WS in H; auto. *) *)
+(*   (*   - rewrite find_val_add_inst; apply WS in H; auto. *) *)
+(*   (*   - rewrite In_fold_left_inst_eq. *) *)
+(*   (*     destruct (ident_eqb x i) eqn: E; *) *)
+(*   (*       [apply ident_eqb_eq in E; subst|apply ident_eqb_neq in E]. *) *)
+(*   (*     + right; apply PSE.MP.Dec.F.add_1; auto. *) *)
+(*   (*     + rewrite find_inst_gso in H; auto. *) *)
+(*   (*       apply WS in H; auto. *) *)
+(*   (*   - destruct (ident_eqb x i) eqn: E; *) *)
+(*   (*       [apply ident_eqb_eq in E; subst|apply ident_eqb_neq in E]. *) *)
+(*   (*     + rewrite find_inst_gss; intro; discriminate. *) *)
+(*   (*     + rewrite find_inst_gso; auto. *) *)
+(*   (*       apply WS. *) *)
+(*   (*       apply In_fold_left_inst_eq in H as [|H]; auto. *) *)
+(*   (*       apply PSE.MP.Dec.F.add_3 in H; auto. *) *)
+(*   (*       contradict H; apply not_In_empty. *) *)
+(*   (* Qed. *) *)
 
-  (* Lemma well_structured_reset_call: *)
-  (*   forall M xs ck f i es ck_r r eqs, *)
-  (*     well_structured_memories (EqCall xs ck f i es :: eqs) M -> *)
-  (*     well_structured_memories (EqReset ck_r f i r :: EqCall xs ck f i es :: eqs) M. *)
-  (* Proof. *)
-  (*   inversion_clear 1 as [Vals Insts]. *)
-  (*   constructor; unfold fbys, insts in *; simpl in *. *)
-  (*   - intro; rewrite Vals; reflexivity. *)
-  (*   - intro; rewrite Insts. *)
-  (*     rewrite 2 In_fold_left_inst_eq. *)
-  (*     split; intros [H|H']; auto. *)
-  (*     + rewrite PSE.MP.Dec.F.add_iff; auto. *)
-  (*     + apply PSE.MP.Dec.F.add_iff in H' as []; auto. *)
-  (*       rewrite PSE.MP.Dec.F.add_iff; auto. *)
-  (* Qed. *)
+(*   (* Lemma well_structured_reset_call: *) *)
+(*   (*   forall M xs ck f i es ck_r r eqs, *) *)
+(*   (*     well_structured_memories (EqCall xs ck f i es :: eqs) M -> *) *)
+(*   (*     well_structured_memories (EqReset ck_r f i r :: EqCall xs ck f i es :: eqs) M. *) *)
+(*   (* Proof. *) *)
+(*   (*   inversion_clear 1 as [Vals Insts]. *) *)
+(*   (*   constructor; unfold fbys, insts in *; simpl in *. *) *)
+(*   (*   - intro; rewrite Vals; reflexivity. *) *)
+(*   (*   - intro; rewrite Insts. *) *)
+(*   (*     rewrite 2 In_fold_left_inst_eq. *) *)
+(*   (*     split; intros [H|H']; auto. *) *)
+(*   (*     + rewrite PSE.MP.Dec.F.add_iff; auto. *) *)
+(*   (*     + apply PSE.MP.Dec.F.add_iff in H' as []; auto. *) *)
+(*   (*       rewrite PSE.MP.Dec.F.add_iff; auto. *) *)
+(*   (* Qed. *) *)
 
-  (* Corollary well_structured_add_inst_reset_call: *)
-  (*   forall M M' xs ck f i es ck_r r eqs, *)
-  (*     well_structured_memories eqs M -> *)
-  (*     well_structured_memories (EqReset ck_r f i r :: EqCall xs ck f i es :: eqs) (add_inst i M' M). *)
-  (* Proof. *)
-  (*   intros; apply well_structured_reset_call, well_structured_add_inst_call; auto. *)
-  (* Qed. *)
+(*   (* Corollary well_structured_add_inst_reset_call: *) *)
+(*   (*   forall M M' xs ck f i es ck_r r eqs, *) *)
+(*   (*     well_structured_memories eqs M -> *) *)
+(*   (*     well_structured_memories (EqReset ck_r f i r :: EqCall xs ck f i es :: eqs) (add_inst i M' M). *) *)
+(*   (* Proof. *) *)
+(*   (*   intros; apply well_structured_reset_call, well_structured_add_inst_call; auto. *) *)
+(*   (* Qed. *) *)
 
-  (* Lemma well_structured_add_val_fby: *)
-  (*   forall M mvs x ck v0 e eqs, *)
-  (*     well_structured_memories eqs M -> *)
-  (*     well_structured_memories (EqFby x ck v0 e :: eqs) (add_val x mvs M). *)
-  (* Proof. *)
-  (*   intros ** WS. *)
-  (*   constructor; unfold fbys, insts; simpl; split; intro H. *)
-  (*   - rewrite In_fold_left_fby_eq. *)
-  (*     destruct (ident_eqb x x0) eqn: E; *)
-  (*       [apply ident_eqb_eq in E; subst|apply ident_eqb_neq in E]. *)
-  (*     + right; apply PSE.MP.Dec.F.add_1; auto. *)
-  (*     + rewrite find_val_gso in H; auto. *)
-  (*       apply WS in H; auto. *)
-  (*   - destruct (ident_eqb x x0) eqn: E; *)
-  (*       [apply ident_eqb_eq in E; subst|apply ident_eqb_neq in E]. *)
-  (*     + rewrite find_val_gss; intro; discriminate. *)
-  (*     + rewrite find_val_gso; auto. *)
-  (*       apply WS. *)
-  (*       apply In_fold_left_fby_eq in H as [|H]; auto. *)
-  (*       apply PSE.MP.Dec.F.add_3 in H; auto. *)
-  (*       contradict H; apply not_In_empty. *)
-  (*   - rewrite find_inst_add_val in H; apply WS in H; auto. *)
-  (*   - rewrite find_inst_add_val; apply WS in H; auto. *)
-  (* Qed. *)
+(*   (* Lemma well_structured_add_val_fby: *) *)
+(*   (*   forall M mvs x ck v0 e eqs, *) *)
+(*   (*     well_structured_memories eqs M -> *) *)
+(*   (*     well_structured_memories (EqFby x ck v0 e :: eqs) (add_val x mvs M). *) *)
+(*   (* Proof. *) *)
+(*   (*   intros ** WS. *) *)
+(*   (*   constructor; unfold fbys, insts; simpl; split; intro H. *) *)
+(*   (*   - rewrite In_fold_left_fby_eq. *) *)
+(*   (*     destruct (ident_eqb x x0) eqn: E; *) *)
+(*   (*       [apply ident_eqb_eq in E; subst|apply ident_eqb_neq in E]. *) *)
+(*   (*     + right; apply PSE.MP.Dec.F.add_1; auto. *) *)
+(*   (*     + rewrite find_val_gso in H; auto. *) *)
+(*   (*       apply WS in H; auto. *) *)
+(*   (*   - destruct (ident_eqb x x0) eqn: E; *) *)
+(*   (*       [apply ident_eqb_eq in E; subst|apply ident_eqb_neq in E]. *) *)
+(*   (*     + rewrite find_val_gss; intro; discriminate. *) *)
+(*   (*     + rewrite find_val_gso; auto. *) *)
+(*   (*       apply WS. *) *)
+(*   (*       apply In_fold_left_fby_eq in H as [|H]; auto. *) *)
+(*   (*       apply PSE.MP.Dec.F.add_3 in H; auto. *) *)
+(*   (*       contradict H; apply not_In_empty. *) *)
+(*   (*   - rewrite find_inst_add_val in H; apply WS in H; auto. *) *)
+(*   (*   - rewrite find_inst_add_val; apply WS in H; auto. *) *)
+(*   (* Qed. *) *)
 
 End SBSEMANTICS.
